<?xml version="1.0"?>

<!DOCTYPE rdf:RDF [
    <!ENTITY owl "http://www.w3.org/2002/07/owl#" >
    <!ENTITY xsd "http://www.w3.org/2001/XMLSchema#" >
    <!ENTITY rdfs "http://www.w3.org/2000/01/rdf-schema#" >
    <!ENTITY rdf "http://www.w3.org/1999/02/22-rdf-syntax-ns#" >
	<!ENTITY foaf "http://xmlns.com/foaf/spec/#" >
	<!ENTITY acdh "https://vocabs.acdh.oeaw.ac.at/#" >
]>

<rdf:RDF xmlns="https://vocabs.acdh.oeaw.ac.at/acdh#"
     xml:base="https://vocabs.acdh.oeaw.ac.at/acdh"
     xmlns:dct="http://purl.org/dc/terms/"
     xmlns:rdf="http://www.w3.org/1999/02/22-rdf-syntax-ns#"
     xmlns:owl="http://www.w3.org/2002/07/owl#"
     xmlns:xml="http://www.w3.org/XML/1998/namespace"
     xmlns:xsd="http://www.w3.org/2001/XMLSchema#"
     xmlns:skos="http://www.w3.org/2004/02/skos/core#"
     xmlns:rdfs="http://www.w3.org/2000/01/rdf-schema#"
     xmlns:acdh="&acdh;"
     xmlns:foaf="http://xmlns.com/foaf/spec/#"
     xmlns:dc="http://purl.org/dc/elements/1.1/">
    <owl:Ontology rdf:about="https://vocabs.acdh.oeaw.ac.at/acdh">
        <owl:versionInfo xml:lang="en">2016-07-26 (Matej) - removed imports </owl:versionInfo>
        <owl:versionInfo xml:lang="en">2017-09-02 (Matej) - reworked definitions for properties, renamed number of properties for consistency, added domains and ranges and inverse properties ; added class Metadata; 
            removed @acdh:hasRelatedMethod@ and @acdh:hasMethod@ in favour of ObjectProperties: @acdh:appliedMethod@/@acdh:methodAppliedIn@ and DataProperty: @acdh:appliedMethodDescription@
        </owl:versionInfo>
        <owl:versionInfo xml:lang="en">2017-10-04 (Martina) Introduced hasCreatedDate for single creation dates. Introduced hasStartDate and hasEndDate for starting and end dates of Projects. Refined some comments for better understanding.</owl:versionInfo>
        <rdfs:comment xml:lang="en">In definitions of properties, &quot;resource A&quot; refers to the subject resource of the property and &quot;resource B&quot; to the object resource</rdfs:comment>
        <owl:versionInfo xml:lang="en">2017-07-18 (Martina, Peter)- all classes and properties assigned with rdfs:label, put under acdh-namespace, flattened Hierarchy</owl:versionInfo>
        <owl:versionInfo xml:lang="en">2016-07-19 (Go) - initial version </owl:versionInfo>
        <rdfs:comment xml:lang="en">When reusing definitions from other vocabularies (esp. DataCite), the reference is given in brackets: (DataCite: ContactPerson). When the source definition was changed slightly the reference is marked with &quot;cf.&quot;</rdfs:comment>
        <owl:versionInfo xml:lang="en">2017-04-06 (Martina) - added cardinality and some test description</owl:versionInfo>
        <owl:versionInfo xml:lang="en">2017-08-24 (Martina)- added comments to all classes and properties with rdfs:comment. Questionable parts marked with &apos;(??)&apos;. </owl:versionInfo>
        <rdfs:comment xml:lang="en">This is the ontology for ACDH repository.</rdfs:comment>
        <owl:versionInfo>2017-06-14 removed and renamed some Digital/Non-Digital classes. 
 DigitalResource -&gt; Resource
 DigitalCollection -&gt; Collection
 DigitalProject -&gt; removed
 rearranged the class hierarchy</owl:versionInfo>
        <owl:versionInfo xml:lang="en">2017-08-27 (Matej) - reworked definitions for classes</owl:versionInfo>
        <rdfs:label>ACDH Schema</rdfs:label>
    </owl:Ontology>
    


    <!-- 
    ///////////////////////////////////////////////////////////////////////////////////////
    //
    // Annotation properties
    //
    ///////////////////////////////////////////////////////////////////////////////////////
     -->

    


    <!-- http://www.w3.org/2000/01/rdf-schema#label -->

    <rdf:Description rdf:about="http://www.w3.org/2000/01/rdf-schema#label">
        <rdfs:label>rdfs:label</rdfs:label>
    </rdf:Description>
    


    <!-- http://www.w3.org/2002/07/owl#inverseOf -->

    <owl:AnnotationProperty rdf:about="http://www.w3.org/2002/07/owl#inverseOf"/>
    


    <!-- http://www.w3.org/2004/02/skos/core#altLabel -->

    <owl:AnnotationProperty rdf:about="http://www.w3.org/2004/02/skos/core#altLabel"/>
    


    <!-- 
    ///////////////////////////////////////////////////////////////////////////////////////
    //
    // Datatypes
    //
    ///////////////////////////////////////////////////////////////////////////////////////
     -->

    


    <!-- http://www.w3.org/2001/XMLSchema#date -->

    <rdfs:Datatype rdf:about="http://www.w3.org/2001/XMLSchema#date"/>
    


    <!-- 
    ///////////////////////////////////////////////////////////////////////////////////////
    //
    // Object Properties
    //
    ///////////////////////////////////////////////////////////////////////////////////////
     -->

    


    <!-- http://purl.org/dc/elements/1.1/contributor -->

    <owl:ObjectProperty rdf:about="http://purl.org/dc/elements/1.1/contributor">
        <owl:equivalentProperty rdf:resource="&acdh;hasContributor"/>
    </owl:ObjectProperty>
    


    <!-- http://purl.org/dc/elements/1.1/coverage -->

    <owl:ObjectProperty rdf:about="http://purl.org/dc/elements/1.1/coverage">
        <owl:equivalentProperty rdf:resource="&acdh;hasSpatialCoverage"/>
    </owl:ObjectProperty>
    


    <!-- http://purl.org/dc/elements/1.1/creator -->

    <owl:ObjectProperty rdf:about="http://purl.org/dc/elements/1.1/creator">
        <owl:equivalentProperty rdf:resource="&acdh;hasCreator"/>
    </owl:ObjectProperty>
    


    <!-- http://purl.org/dc/elements/1.1/format -->

    <owl:ObjectProperty rdf:about="http://purl.org/dc/elements/1.1/format">
        <owl:equivalentProperty rdf:resource="&acdh;hasFormat"/>
    </owl:ObjectProperty>
    


    <!-- http://purl.org/dc/elements/1.1/publisher -->

    <owl:ObjectProperty rdf:about="http://purl.org/dc/elements/1.1/publisher">
        <owl:equivalentProperty rdf:resource="&acdh;hasHosting"/>
    </owl:ObjectProperty>
    


    <!-- http://purl.org/dc/elements/1.1/relation -->

    <owl:ObjectProperty rdf:about="http://purl.org/dc/elements/1.1/relation">
        <owl:equivalentProperty rdf:resource="&acdh;hasRelatedProject"/>
        <owl:equivalentProperty rdf:resource="&acdh;relation"/>
    </owl:ObjectProperty>
    


    <!-- http://purl.org/dc/elements/1.1/rights -->

    <owl:ObjectProperty rdf:about="http://purl.org/dc/elements/1.1/rights">
        <owl:equivalentProperty rdf:resource="&acdh;hasLicense"/>
    </owl:ObjectProperty>
    


    <!-- http://purl.org/dc/elements/1.1/source -->

    <owl:ObjectProperty rdf:about="http://purl.org/dc/elements/1.1/source">
        <owl:equivalentProperty rdf:resource="&acdh;hasSource"/>
    </owl:ObjectProperty>
    


    <!-- http://purl.org/dc/elements/1.1/subject -->

    <owl:ObjectProperty rdf:about="http://purl.org/dc/elements/1.1/subject">
        <owl:equivalentProperty rdf:resource="&acdh;hasSubject"/>
    </owl:ObjectProperty>
    


    <!-- http://purl.org/dc/elements/1.1/type -->

    <owl:ObjectProperty rdf:about="http://purl.org/dc/elements/1.1/type">
        <owl:equivalentProperty rdf:resource="&acdh;hasCategory"/>
    </owl:ObjectProperty>
    


    <!-- &acdh;cites -->

    <owl:ObjectProperty rdf:about="&acdh;cites">
        <rdfs:subPropertyOf rdf:resource="&acdh;relation"/>
        <owl:inverseOf rdf:resource="&acdh;isCitedBy"/>
        <rdfs:domain rdf:resource="&acdh;RepoObject"/>
        <rdfs:range rdf:resource="&acdh;RepoObject"/>
        <rdfs:comment xml:lang="en">Indicates that A refers to B in a citation.</rdfs:comment>
        <rdfs:label xml:lang="en">cites</rdfs:label>
        <skos:altLabel xml:lang="en">Cites</skos:altLabel>
        <skos:altLabel xml:lang="de">Zitiert</skos:altLabel>
    </owl:ObjectProperty>
    


    <!-- &acdh;compiles -->

    <owl:ObjectProperty rdf:about="&acdh;compiles">
        <rdfs:subPropertyOf rdf:resource="&acdh;relation"/>
        <owl:inverseOf rdf:resource="&acdh;isCompiledBy"/>
        <rdfs:domain rdf:resource="&acdh;RepoObject"/>
        <rdfs:range rdf:resource="&acdh;RepoObject"/>
        <rdfs:comment xml:lang="en">Indicates B is the result of a compile or creation event using A.</rdfs:comment>
        <rdfs:label xml:lang="en">compiles</rdfs:label>
        <skos:altLabel xml:lang="en">Compiles</skos:altLabel>
        <skos:altLabel xml:lang="de">Stellt zusammen</skos:altLabel>
    </owl:ObjectProperty>
    


    <!-- &acdh;continues -->

    <owl:ObjectProperty rdf:about="&acdh;continues">
        <rdfs:subPropertyOf rdf:resource="&acdh;relation"/>
        <owl:inverseOf rdf:resource="&acdh;isContinuedBy"/>
        <rdfs:domain rdf:resource="&acdh;RepoObject"/>
        <rdfs:range rdf:resource="&acdh;RepoObject"/>
        <rdfs:comment xml:lang="en">Indicates A is a continuation of the work B.</rdfs:comment>
        <rdfs:label xml:lang="en">continues</rdfs:label>
        <skos:altLabel xml:lang="en">Continues</skos:altLabel>
        <skos:altLabel xml:lang="de">Setzt fort</skos:altLabel>
    </owl:ObjectProperty>
    


    <!-- &acdh;documents -->

    <owl:ObjectProperty rdf:about="&acdh;documents">
        <rdfs:subPropertyOf rdf:resource="&acdh;relation"/>
        <owl:inverseOf rdf:resource="&acdh;isDocumentedBy"/>
        <rdfs:domain rdf:resource="&acdh;RepoObject"/>
        <rdfs:range rdf:resource="&acdh;RepoObject"/>
        <rdfs:comment xml:lang="en">Indicates A is documentation about B.</rdfs:comment>
        <rdfs:label xml:lang="en">documents</rdfs:label>
        <skos:altLabel xml:lang="en">Documents</skos:altLabel>
        <skos:altLabel xml:lang="de">Dokumentiert</skos:altLabel>
    </owl:ObjectProperty>
    


    <!-- &acdh;hasAccessRestriction -->

    <owl:ObjectProperty rdf:about="&acdh;hasAccessRestriction">
        <rdfs:subPropertyOf rdf:resource="http://www.w3.org/2002/07/owl#topObjectProperty"/>
        <owl:inverseOf rdf:resource="&acdh;isAccessRestriction"/>
        <rdfs:domain rdf:resource="&acdh;RepoObject"/>
        <rdfs:comment xml:lang="en">Denotes if restricted access applies to the Resource (A).</rdfs:comment>
        <rdfs:comment xml:lang="en">[Matej: what is the range of the property? Why is it object property? ??]</rdfs:comment>
        <rdfs:label xml:lang="en">has access restriction</rdfs:label>
        <skos:altLabel xml:lang="en">Has access restriction</skos:altLabel>
        <skos:altLabel xml:lang="de">Hat Zugriffsbeschränkung</skos:altLabel>
    </owl:ObjectProperty>
    


    <!-- &acdh;hasActor -->

    <owl:ObjectProperty rdf:about="&acdh;hasActor">
        <rdfs:subPropertyOf rdf:resource="&acdh;hasCoverage"/>
        <owl:inverseOf rdf:resource="&acdh;isActor"/>
        <rdfs:domain rdf:resource="&acdh;RepoObject"/>
        <rdfs:range rdf:resource="&acdh;Agent"/>
        <rdfs:comment xml:lang="en">Any person or institution (B) which the given resource (A) mentions or is about.</rdfs:comment>
        <rdfs:label xml:lang="en">has actor</rdfs:label>
        <skos:altLabel xml:lang="en">Has actor</skos:altLabel>
        <skos:altLabel xml:lang="de">Hat Akteur</skos:altLabel>
    </owl:ObjectProperty>
    


    <!-- &acdh;hasAppliedMethod -->

    <owl:ObjectProperty rdf:about="&acdh;hasAppliedMethod">
        <rdfs:subPropertyOf rdf:resource="http://www.w3.org/2002/07/owl#topObjectProperty"/>
        <owl:inverseOf rdf:resource="&acdh;isAppliedMethod"/>
        <rdfs:range rdf:resource="&acdh;Concept"/>
        <rdfs:comment xml:lang="en">The methodology (B) applied in creation or curation of the resource or in the project (A) (cf. DataCite: descriptionType methods) </rdfs:comment>
        <rdfs:label xml:lang="en">has applied method</rdfs:label>
        <rdfs:seeAlso>acdh:appliedMethodDescription a owl:DatatypeProperty</rdfs:seeAlso>
        <skos:altLabel xml:lang="de">Angewandte Methode</skos:altLabel>
        <skos:altLabel xml:lang="en">Applied method</skos:altLabel>
    </owl:ObjectProperty>
    


    <!-- &acdh;hasAuthor -->

    <owl:ObjectProperty rdf:about="&acdh;hasAuthor">
        <rdfs:subPropertyOf rdf:resource="&acdh;hasCreator"/>
        <owl:inverseOf rdf:resource="&acdh;isAuthor"/>
        <rdfs:domain rdf:resource="&acdh;RepoObject"/>
        <rdfs:range rdf:resource="&acdh;Agent"/>
        <rdfs:comment xml:lang="en">Author of resource, who will appear in the citation of it.</rdfs:comment>
        <rdfs:comment xml:lang="en">[(??) Has to be distinguished more clearly from creator.]</rdfs:comment>
        <rdfs:label xml:lang="en">has author</rdfs:label>
        <skos:altLabel xml:lang="en">Has author</skos:altLabel>
        <skos:altLabel xml:lang="de">Hat Autor</skos:altLabel>
    </owl:ObjectProperty>
    


    <!-- &acdh;hasCategory -->

    <owl:ObjectProperty rdf:about="&acdh;hasCategory">
        <rdfs:subPropertyOf rdf:resource="http://www.w3.org/2002/07/owl#topObjectProperty"/>
        <owl:inverseOf rdf:resource="&acdh;isCategory"/>
        <rdfs:domain rdf:resource="&acdh;RepoObject"/>
        <rdfs:range rdf:resource="&acdh;Concept"/>
        <rdfs:comment xml:lang="en">Type of resource, e. g. corpus. Choose from list. Can be refined with description, format, extent, etc.</rdfs:comment>
        <rdfs:comment>[just for resource type, with controlled vocabulary]</rdfs:comment>
        <rdfs:label xml:lang="en">has category</rdfs:label>
        <skos:altLabel xml:lang="en">Has category</skos:altLabel>
        <skos:altLabel xml:lang="de">Hat Kategorie</skos:altLabel>
    </owl:ObjectProperty>
    


    <!-- &acdh;hasContact -->

    <owl:ObjectProperty rdf:about="&acdh;hasContact">
        <rdfs:subPropertyOf rdf:resource="&acdh;hasContributor"/>
        <owl:inverseOf rdf:resource="&acdh;isContact"/>
        <rdfs:range rdf:resource="&acdh;Agent"/>
        <rdfs:comment xml:lang="en">Person or Organisation (B) that can be contacted regarding information about a Resource or a Project (A).</rdfs:comment>
        <rdfs:comment xml:lang="en">Person with knowledge of how to access, troubleshoot, or otherwise field issues related to the resource. (DataCite: ContactPerson)</rdfs:comment>
        <rdfs:label xml:lang="en">has contact</rdfs:label>
        <skos:altLabel xml:lang="en">Has contact</skos:altLabel>
        <skos:altLabel xml:lang="de">Hat Kontakt</skos:altLabel>
    </owl:ObjectProperty>
    


    <!-- &acdh;hasContributor -->

    <owl:ObjectProperty rdf:about="&acdh;hasContributor">
        <rdfs:subPropertyOf rdf:resource="http://www.w3.org/2002/07/owl#topObjectProperty"/>
        <owl:inverseOf rdf:resource="&acdh;isContributor"/>
        <rdfs:range rdf:resource="&acdh;Agent"/>
        <rdfs:comment xml:lang="en">Agent (person, group, organisation) (B) who was actively involved in creating/curating/editing a Resource, a Collection or in a Project (A). Any person or institution making a significant contribution to the development and/or maintenance of the resource, but whose contribution does not “fit” to another already defined role. (cf. DataCite: Other)
This is a generic property. Use one of the more specific sub-properties where possible.</rdfs:comment>
        <rdfs:label xml:lang="en">has contributor</rdfs:label>
        <skos:altLabel xml:lang="en">Has contributor</skos:altLabel>
        <skos:altLabel xml:lang="de">Hat Mitarbeiter oder Beitragenden</skos:altLabel>
    </owl:ObjectProperty>
    


    <!-- &acdh;hasCoverage -->

    <owl:ObjectProperty rdf:about="&acdh;hasCoverage">
        <rdfs:subPropertyOf rdf:resource="http://www.w3.org/2002/07/owl#topObjectProperty"/>
        <owl:inverseOf rdf:resource="&acdh;isCoverage"/>
        <rdfs:range rdf:resource="&acdh;Concept"/>
        <rdfs:comment xml:lang="en">Generic indication of what is covered/mentioned in the resource  (its content) along various dimensions (subject, space, time). Use the more specific sub-properties where possible.</rdfs:comment>
        <rdfs:label xml:lang="en">has coverage</rdfs:label>
        <owl:inverseOf></owl:inverseOf>
        <skos:altLabel xml:lang="de">Deckt ab</skos:altLabel>
        <skos:altLabel xml:lang="en">Has coverage</skos:altLabel>
    </owl:ObjectProperty>
    


    <!-- &acdh;hasCreator -->

    <owl:ObjectProperty rdf:about="&acdh;hasCreator">
        <rdfs:subPropertyOf rdf:resource="&acdh;hasContributor"/>
        <owl:inverseOf rdf:resource="&acdh;isCreator"/>
        <rdfs:domain rdf:resource="&acdh;RepoObject"/>
        <rdfs:range rdf:resource="&acdh;Agent"/>
        <rdfs:comment xml:lang="en">Person (B) responsible for creation of resource (A).</rdfs:comment>
        <rdfs:label xml:lang="en">has creator</rdfs:label>
        <skos:altLabel xml:lang="en">Has creator</skos:altLabel>
        <skos:altLabel xml:lang="de">Hat Urheber</skos:altLabel>
    </owl:ObjectProperty>
    


    <!-- &acdh;hasCurator -->

    <owl:ObjectProperty rdf:about="&acdh;hasCurator">
        <rdfs:subPropertyOf rdf:resource="&acdh;hasContributor"/>
        <owl:inverseOf rdf:resource="&acdh;isCurator"/>
        <rdfs:domain rdf:resource="&acdh;RepoObject"/>
        <rdfs:range rdf:resource="&acdh;Agent"/>
        <rdfs:comment xml:lang="en">Person (B) tasked with reviewing, enhancing, cleaning, or standardizing data and the associated metadata submitted for storage, use, and maintenance within a data centre or repository. (cf. DataCite: DataCurator)</rdfs:comment>
        <rdfs:label xml:lang="en">has curator</rdfs:label>
        <skos:altLabel xml:lang="en">Has data curator</skos:altLabel>
        <skos:altLabel xml:lang="de">Hat Datenkurator</skos:altLabel>
    </owl:ObjectProperty>
    


    <!-- &acdh;hasDepositor -->

    <owl:ObjectProperty rdf:about="&acdh;hasDepositor">
        <rdfs:subPropertyOf rdf:resource="&acdh;hasContributor"/>
        <owl:inverseOf rdf:resource="&acdh;isDepositor"/>
        <rdfs:domain rdf:resource="&acdh;RepoObject"/>
        <rdfs:range rdf:resource="&acdh;Agent"/>
        <rdfs:comment xml:lang="en">Person or organisation (B) responsible for submitting a resource (A) for hosting to the repository.</rdfs:comment>
        <rdfs:label xml:lang="en">has depositor</rdfs:label>
        <skos:altLabel xml:lang="en">Has depositor</skos:altLabel>
        <skos:altLabel xml:lang="de">Hat Datengeber</skos:altLabel>
    </owl:ObjectProperty>
    


    <!-- &acdh;hasDerivedPublication -->

    <owl:ObjectProperty rdf:about="&acdh;hasDerivedPublication">
        <rdfs:subPropertyOf rdf:resource="&acdh;relation"/>
        <owl:inverseOf rdf:resource="&acdh;isDerivedPublication"/>
        <rdfs:range rdf:resource="&acdh;Publication"/>
        <rdfs:comment xml:lang="en">A publication derived from a project, collection or even resource.</rdfs:comment>
        <rdfs:label xml:lang="en">has derived publication</rdfs:label>
        <skos:altLabel xml:lang="en">Has derived publication</skos:altLabel>
        <skos:altLabel xml:lang="de">Hat abgeleitete Publikation</skos:altLabel>
    </owl:ObjectProperty>
    


    <!-- &acdh;hasEditor -->

    <owl:ObjectProperty rdf:about="&acdh;hasEditor">
        <rdfs:subPropertyOf rdf:resource="&acdh;hasContributor"/>
        <owl:inverseOf rdf:resource="&acdh;isEditor"/>
        <rdfs:domain rdf:resource="&acdh;RepoObject"/>
        <rdfs:range rdf:resource="&acdh;Agent"/>
        <rdfs:comment xml:lang="en">A person who oversees the details related to the publication format of the resource. (DataCite Editor)</rdfs:comment>
        <rdfs:label xml:lang="en">has editor</rdfs:label>
        <skos:altLabel xml:lang="en">Has editor</skos:altLabel>
        <skos:altLabel xml:lang="de">Hat Herausgeber</skos:altLabel>
    </owl:ObjectProperty>
    


    <!-- &acdh;hasFormat -->

    <owl:ObjectProperty rdf:about="&acdh;hasFormat">
        <rdfs:subPropertyOf rdf:resource="http://www.w3.org/2002/07/owl#topObjectProperty"/>
        <owl:inverseOf rdf:resource="&acdh;isFormat"/>
        <rdfs:domain rdf:resource="&acdh;Resource"/>
        <rdfs:comment xml:lang="en">Format of a resource (A). Indicated as MIME type.</rdfs:comment>
        <rdfs:comment xml:lang="en">[Matej: What is the range of the property? The MIME types, but how do you refer to these. Shouldn&apos;t this be a DatatypeProperty with a controlled vocabulary ??]</rdfs:comment>
        <rdfs:label xml:lang="en">has format</rdfs:label>
        <skos:altLabel xml:lang="en">Has format</skos:altLabel>
        <skos:altLabel xml:lang="de">Hat Format</skos:altLabel>
    </owl:ObjectProperty>
    


    <!-- &acdh;hasFunder -->

    <owl:ObjectProperty rdf:about="&acdh;hasFunder">
        <rdfs:subPropertyOf rdf:resource="&acdh;hasContributor"/>
        <owl:inverseOf rdf:resource="&acdh;isFunder"/>
        <rdfs:domain rdf:resource="&acdh;Project"/>
        <rdfs:range rdf:resource="&acdh;Agent"/>
        <rdfs:comment xml:lang="en">Person or Organisation (B) which provided funding for the project (A). </rdfs:comment>
        <rdfs:comment xml:lang="en">Person or organisation that issued a contract or under the auspices of which a work has been written, printed, published, developed, etc. (DataCite: Sponsor)</rdfs:comment>
        <rdfs:label xml:lang="en">has funder</rdfs:label>
        <skos:altLabel xml:lang="en">Has funder</skos:altLabel>
        <skos:altLabel xml:lang="de">Hat Geldgeber</skos:altLabel>
    </owl:ObjectProperty>
    


    <!-- &acdh;hasHosting -->

    <owl:ObjectProperty rdf:about="&acdh;hasHosting">
        <rdfs:subPropertyOf rdf:resource="&acdh;hasContributor"/>
        <owl:inverseOf rdf:resource="&acdh;isHosting"/>
        <rdfs:domain rdf:resource="&acdh;RepoObject"/>
        <rdfs:range rdf:resource="&acdh;Agent"/>
        <rdfs:comment xml:lang="en">Institution responsible for preservation/hosting of a resource. (DataCite: HostingInstitution) Typically, the organisation allowing the resource to be available on the internet through the provision of its hardware/software/operating support.</rdfs:comment>
        <rdfs:label xml:lang="en">has hosting</rdfs:label>
        <skos:altLabel xml:lang="en">Has host</skos:altLabel>
        <skos:altLabel xml:lang="de">Wird erhalten/bereitgestellt von</skos:altLabel>
    </owl:ObjectProperty>
    


    <!-- &acdh;hasLicense -->

    <owl:ObjectProperty rdf:about="&acdh;hasLicense">
        <rdfs:subPropertyOf rdf:resource="http://www.w3.org/2002/07/owl#topObjectProperty"/>
        <owl:inverseOf rdf:resource="&acdh;isLicense"/>
        <rdfs:domain rdf:resource="&acdh;RepoObject"/>
        <rdfs:comment xml:lang="en">Denotes the license attached to an object.</rdfs:comment>
        <rdfs:label xml:lang="en">has license</rdfs:label>
        <skos:altLabel xml:lang="en">Has license</skos:altLabel>
        <skos:altLabel xml:lang="de">Hat Lizenz</skos:altLabel>
    </owl:ObjectProperty>
    


    <!-- &acdh;hasLicensor -->

    <owl:ObjectProperty rdf:about="&acdh;hasLicensor">
        <rdfs:subPropertyOf rdf:resource="&acdh;hasContributor"/>
        <owl:inverseOf rdf:resource="&acdh;isLicensor"/>
        <rdfs:domain rdf:resource="&acdh;RepoObject"/>
        <rdfs:range rdf:resource="&acdh;Agent"/>
        <rdfs:comment xml:lang="en">Person or Organisation responsible for choosing a license for the Object.</rdfs:comment>
        <rdfs:label xml:lang="en">has licensor</rdfs:label>
        <skos:altLabel xml:lang="en">Has licensor</skos:altLabel>
        <skos:altLabel xml:lang="de">Hat Lizenzgeber</skos:altLabel>
    </owl:ObjectProperty>
    


    <!-- &acdh;hasLifeCycleStatus -->

    <owl:ObjectProperty rdf:about="&acdh;hasLifeCycleStatus">
        <rdfs:subPropertyOf rdf:resource="http://www.w3.org/2002/07/owl#topObjectProperty"/>
        <owl:inverseOf rdf:resource="&acdh;isLifeCycleStatus"/>
        <rdfs:comment xml:lang="en">Indication if the Project, Collection or Resource (A) still in the making or completed? A verbose status description can be added with acdh:hasCompleteness.</rdfs:comment>
        <rdfs:comment xml:lang="en">[Matej: define allowed values as controlled vocabulary. !!]</rdfs:comment>
        <rdfs:label xml:lang="en">has life cycle status</rdfs:label>
        <skos:altLabel xml:lang="en">Has life cycle status</skos:altLabel>
        <skos:altLabel xml:lang="de">Hat Lebenszyklusstatus</skos:altLabel>
    </owl:ObjectProperty>
    


    <!-- &acdh;hasMember -->

    <owl:ObjectProperty rdf:about="&acdh;hasMember">
        <owl:inverseOf rdf:resource="&acdh;isMember"/>
        <rdfs:range rdf:resource="&acdh;Agent"/>
        <rdfs:comment xml:lang="en">Used to link a Person to an Organisation or an Organisation (e.g. department) to another Organisation (institution)</rdfs:comment>
        <rdfs:label xml:lang="en">has member</rdfs:label>
        <skos:altLabel xml:lang="en">Has member</skos:altLabel>
        <skos:altLabel xml:lang="de">Hat Mitglied</skos:altLabel>
    </owl:ObjectProperty>
    


    <!-- &acdh;hasMetadata -->

    <owl:ObjectProperty rdf:about="&acdh;hasMetadata">
        <rdfs:subPropertyOf rdf:resource="&acdh;relation"/>
        <owl:inverseOf rdf:resource="&acdh;isMetadataFor"/>
        <rdfs:domain rdf:resource="&acdh;RepoObject"/>
        <rdfs:range rdf:resource="&acdh;Metadata"/>
        <rdfs:comment xml:lang="en">Resource B describes / is about resource A.</rdfs:comment>
        <rdfs:label xml:lang="en">has metadata</rdfs:label>
        <skos:altLabel xml:lang="en">Has metadata</skos:altLabel>
        <skos:altLabel xml:lang="de">Hat Metadaten</skos:altLabel>
    </owl:ObjectProperty>
    


    <!-- &acdh;hasMetadataCreator -->

    <owl:ObjectProperty rdf:about="&acdh;hasMetadataCreator">
        <rdfs:subPropertyOf rdf:resource="&acdh;hasContributor"/>
        <owl:inverseOf rdf:resource="&acdh;isMetadataCreator"/>
        <rdfs:domain rdf:resource="&acdh;RepoObject"/>
        <rdfs:range rdf:resource="&acdh;Agent"/>
        <rdfs:comment xml:lang="en">Person or Organisation responsible for creating metadata for a Resource or Collection.</rdfs:comment>
        <rdfs:comment>[Martina: do we need both inverse properties?]</rdfs:comment>
        <rdfs:label xml:lang="en">has metadata creator</rdfs:label>
        <skos:altLabel xml:lang="en">Has metadata creator</skos:altLabel>
        <skos:altLabel xml:lang="de">Hat Metadatenersteller</skos:altLabel>
    </owl:ObjectProperty>
    


    <!-- &acdh;hasOwner -->

    <owl:ObjectProperty rdf:about="&acdh;hasOwner">
        <rdfs:subPropertyOf rdf:resource="&acdh;hasContributor"/>
        <owl:inverseOf rdf:resource="&acdh;isOwner"/>
        <rdfs:domain rdf:resource="&acdh;RepoObject"/>
        <rdfs:range rdf:resource="&acdh;Agent"/>
        <rdfs:comment xml:lang="en">Person or Organisation who owns given Collection or Resource.</rdfs:comment>
        <rdfs:label xml:lang="en">has owner</rdfs:label>
        <skos:altLabel xml:lang="en">Has owner</skos:altLabel>
        <skos:altLabel xml:lang="de">Hat Besitzer</skos:altLabel>
    </owl:ObjectProperty>
    


    <!-- &acdh;hasPart -->

    <owl:ObjectProperty rdf:about="&acdh;hasPart">
        <rdfs:subPropertyOf rdf:resource="&acdh;relation"/>
        <owl:inverseOf rdf:resource="&acdh;isPartOf"/>
        <rdfs:domain rdf:resource="&acdh;Collection"/>
        <rdfs:range rdf:resource="&acdh;RepoObject"/>
        <rdfs:comment xml:lang="en">Indicates B is part of / member of A, e. g. elements of a series.</rdfs:comment>
        <rdfs:label xml:lang="en">has part</rdfs:label>
        <skos:altLabel xml:lang="en">Has part</skos:altLabel>
        <skos:altLabel xml:lang="de">Hat Teil</skos:altLabel>
    </owl:ObjectProperty>
    


    <!-- &acdh;hasPrincipalInvestigator -->

    <owl:ObjectProperty rdf:about="&acdh;hasPrincipalInvestigator">
        <rdfs:subPropertyOf rdf:resource="&acdh;hasContributor"/>
        <owl:inverseOf rdf:resource="&acdh;isPrincipalInvestigator"/>
        <rdfs:domain rdf:resource="&acdh;Project"/>
        <rdfs:range rdf:resource="&acdh;Agent"/>
        <rdfs:comment xml:lang="en">Person officially designated as head of project team or subproject team instrumental in the work necessary to development of the resource. (DataCite: ProjectLeader)</rdfs:comment>
        <rdfs:label xml:lang="en">has principal investigator</rdfs:label>
        <skos:altLabel xml:lang="en">Has principal investigator</skos:altLabel>
        <skos:altLabel xml:lang="de">Hat Primärforscher</skos:altLabel>
    </owl:ObjectProperty>
    


    <!-- &acdh;hasPublicationPlace -->

    <owl:ObjectProperty rdf:about="&acdh;hasPublicationPlace">
        <owl:inverseOf rdf:resource="&acdh;isPublicationPlace"/>
        <rdfs:comment xml:lang="en">Connects a Publication with a Place, where it was published.</rdfs:comment>
        <rdfs:label xml:lang="en">has publication place</rdfs:label>
        <skos:altLabel xml:lang="en">Publication place</skos:altLabel>
        <skos:altLabel xml:lang="de">Veröffentlichungsort</skos:altLabel>
    </owl:ObjectProperty>
    


    <!-- &acdh;hasRelatedCollection -->

    <owl:ObjectProperty rdf:about="&acdh;hasRelatedCollection">
        <rdfs:subPropertyOf rdf:resource="&acdh;relation"/>
        <owl:inverseOf rdf:resource="&acdh;hasRelatedProject"/>
        <rdfs:domain rdf:resource="&acdh;Project"/>
        <rdfs:range rdf:resource="&acdh;Collection"/>
        <rdfs:comment xml:lang="en">Indication of collection associated to this project.</rdfs:comment>
        <rdfs:comment>[http used instead of https]</rdfs:comment>
        <rdfs:label xml:lang="en">has related collection</rdfs:label>
        <skos:altLabel xml:lang="en">Related collection</skos:altLabel>
        <skos:altLabel xml:lang="de">Zugehörige Sammlung</skos:altLabel>
    </owl:ObjectProperty>
    


    <!-- &acdh;hasRelatedDiscipline -->

    <owl:ObjectProperty rdf:about="&acdh;hasRelatedDiscipline">
        <rdfs:subPropertyOf rdf:resource="http://www.w3.org/2002/07/owl#topObjectProperty"/>
        <owl:inverseOf rdf:resource="&acdh;isRelatedDiscipline"/>
        <rdfs:domain rdf:resource="&acdh;RepoObject"/>
        <rdfs:range rdf:resource="&acdh;Concept"/>
        <rdfs:comment xml:lang="en">Discipline of Project, Collection or Resource. Can be used for search. </rdfs:comment>
        <rdfs:comment>[Martina: should this be a sub of relation?]</rdfs:comment>
        <rdfs:comment>[Matej: review definition! ??]</rdfs:comment>
        <rdfs:label xml:lang="en">has related discipline</rdfs:label>
        <skos:altLabel xml:lang="en">Has related discipline</skos:altLabel>
        <skos:altLabel xml:lang="de">Hat zugehörige Disziplin</skos:altLabel>
    </owl:ObjectProperty>
    


    <!-- &acdh;hasRelatedProject -->

    <owl:ObjectProperty rdf:about="&acdh;hasRelatedProject">
        <rdfs:subPropertyOf rdf:resource="&acdh;relation"/>
        <rdfs:domain rdf:resource="&acdh;RepoObject"/>
        <rdfs:range rdf:resource="&acdh;Project"/>
        <rdfs:comment xml:lang="en">Indication of a project (B) associated with this resource or collection (A).</rdfs:comment>
        <rdfs:comment>[Martina: should this be a sub of relation?]</rdfs:comment>
        <rdfs:label xml:lang="en">has related project</rdfs:label>
        <skos:altLabel xml:lang="en">Has related project</skos:altLabel>
        <skos:altLabel xml:lang="de">Hat zugehöriges Projekt</skos:altLabel>
    </owl:ObjectProperty>
    


    <!-- &acdh;hasRightsHolder -->

    <owl:ObjectProperty rdf:about="&acdh;hasRightsHolder">
        <rdfs:subPropertyOf rdf:resource="&acdh;hasContributor"/>
        <owl:inverseOf rdf:resource="&acdh;isRightsHolder"/>
        <rdfs:domain rdf:resource="&acdh;RepoObject"/>
        <rdfs:range rdf:resource="&acdh;Agent"/>
        <rdfs:comment xml:lang="en">Person or institution (B) owning or managing property rights, including intellectual property rights over the resource (A). (DataCite RightsHolder)</rdfs:comment>
        <rdfs:label xml:lang="en">has rights holder</rdfs:label>
        <skos:altLabel xml:lang="en">Has rights holder</skos:altLabel>
        <skos:altLabel xml:lang="de">Hat Rechteinhaber</skos:altLabel>
    </owl:ObjectProperty>
    


    <!-- &acdh;hasSchema -->

    <owl:ObjectProperty rdf:about="&acdh;hasSchema">
        <rdfs:subPropertyOf rdf:resource="http://www.w3.org/2002/07/owl#topObjectProperty"/>
        <owl:inverseOf rdf:resource="&acdh;isSchema"/>
        <rdfs:domain rdf:resource="&acdh;Resource"/>
        <rdfs:range rdf:resource="&acdh;Resource"/>
        <rdfs:comment xml:lang="en">Reference to a definition of the structure of the resource (A). This could be a XML schema, a SQL-DB definition an ontology, etc.</rdfs:comment>
        <rdfs:label xml:lang="en">has schema</rdfs:label>
        <skos:altLabel xml:lang="en">Has schema</skos:altLabel>
        <skos:altLabel xml:lang="de">Hat Schema</skos:altLabel>
    </owl:ObjectProperty>
    


    <!-- &acdh;hasSource -->

    <owl:ObjectProperty rdf:about="&acdh;hasSource">
        <rdfs:subPropertyOf rdf:resource="&acdh;relation"/>
        <owl:inverseOf rdf:resource="&acdh;isSourceOf"/>
        <rdfs:domain rdf:resource="&acdh;Resource"/>
        <rdfs:range rdf:resource="&acdh;Resource"/>
        <rdfs:comment xml:lang="en">Indicates A is based on source B.</rdfs:comment>
        <rdfs:label xml:lang="en">has source</rdfs:label>
        <skos:altLabel xml:lang="en">Has source</skos:altLabel>
        <skos:altLabel xml:lang="de">Hat Quelle</skos:altLabel>
    </owl:ObjectProperty>
    


    <!-- &acdh;hasSpatialCoverage -->

    <owl:ObjectProperty rdf:about="&acdh;hasSpatialCoverage">
        <rdfs:subPropertyOf rdf:resource="&acdh;hasCoverage"/>
        <owl:inverseOf rdf:resource="&acdh;isSpatialCoverage"/>
        <rdfs:range rdf:resource="&acdh;Place"/>
        <rdfs:comment xml:lang="en">Geographical location, area, region (B) a Project, Collection or Resource (A) is dealing with, is about; e.g. archaeological data from excavations in &apos;Pannonia&apos; or a collection of digitised newspapers from &apos;Austria&apos;.</rdfs:comment>
        <rdfs:label xml:lang="en">has spatial coverage</rdfs:label>
        <skos:altLabel xml:lang="en">Has spatial coverage</skos:altLabel>
        <skos:altLabel xml:lang="de">Hat geografische Abdeckung</skos:altLabel>
    </owl:ObjectProperty>
    


    <!-- &acdh;hasSubject -->

    <owl:ObjectProperty rdf:about="&acdh;hasSubject">
        <rdfs:subPropertyOf rdf:resource="&acdh;hasCoverage"/>
        <owl:inverseOf rdf:resource="&acdh;isSubject"/>
        <rdfs:range rdf:resource="&acdh;Concept"/>
        <rdfs:comment xml:lang="en">Subject of Project, Collection or Resource. Can be used as keywords for search.</rdfs:comment>
        <rdfs:label xml:lang="en">has subject</rdfs:label>
        <skos:altLabel xml:lang="en">Has subject</skos:altLabel>
        <skos:altLabel xml:lang="de">Hat Gegenstand</skos:altLabel>
    </owl:ObjectProperty>
    


    <!-- &acdh;hasTitleImage -->

    <owl:ObjectProperty rdf:about="&acdh;hasTitleImage">
        <rdfs:subPropertyOf rdf:resource="&acdh;relation"/>
        <owl:inverseOf rdf:resource="&acdh;isTitleImageOf"/>
        <rdfs:domain rdf:resource="&acdh;RepoObject"/>
        <rdfs:range rdf:resource="&acdh;Image"/>
        <rdfs:comment xml:lang="en">Title image or logo of Organisation, Project Collection or Resource used for presentation.</rdfs:comment>
        <rdfs:label xml:lang="en">has title image</rdfs:label>
        <skos:altLabel xml:lang="en">Has title image</skos:altLabel>
        <skos:altLabel xml:lang="de">Hat Titelbild</skos:altLabel>
    </owl:ObjectProperty>
    


    <!-- &acdh;hasTransferMethod -->

    <owl:ObjectProperty rdf:about="&acdh;hasTransferMethod">
        <rdfs:subPropertyOf rdf:resource="http://www.w3.org/2002/07/owl#topObjectProperty"/>
        <owl:inverseOf rdf:resource="&acdh;isTransferMethod"/>
        <rdfs:domain rdf:resource="&acdh;RepoObject"/>
        <rdfs:range rdf:resource="&acdh;Concept"/>
        <rdfs:comment xml:lang="en">Method used to transfer resources from depositor to repository.</rdfs:comment>
        <rdfs:comment xml:lang="en">[Matej: needs controlled vocabulary!!]</rdfs:comment>
        <rdfs:label xml:lang="en">has transfer method</rdfs:label>
        <skos:altLabel xml:lang="en">Has transfer method</skos:altLabel>
        <skos:altLabel xml:lang="de">Hat Transfermethode</skos:altLabel>
    </owl:ObjectProperty>
    


    <!-- &acdh;isAccessRestriction -->

    <owl:ObjectProperty rdf:about="&acdh;isAccessRestriction">
        <rdfs:subPropertyOf rdf:resource="http://www.w3.org/2002/07/owl#topObjectProperty"/>
        <rdfs:range rdf:resource="&acdh;RepoObject"/>
        <rdfs:comment xml:lang="en">Denotes if restricted access applies to the Resource.</rdfs:comment>
        <rdfs:comment>[Martina: rename to isAccessRestriction]</rdfs:comment>
        <rdfs:label xml:lang="en">is access restriction</rdfs:label>
        <skos:altLabel xml:lang="en">Restricted access</skos:altLabel>
        <skos:altLabel xml:lang="de">Zugriffsbeschränkung</skos:altLabel>
    </owl:ObjectProperty>
    


    <!-- &acdh;isActor -->

    <owl:ObjectProperty rdf:about="&acdh;isActor">
        <rdfs:subPropertyOf rdf:resource="&acdh;isCoverage"/>
        <rdfs:domain rdf:resource="&acdh;Agent"/>
        <rdfs:comment xml:lang="en">Any person or institution (A) which the given resource (B) mentions or is about.</rdfs:comment>
        <rdfs:label xml:lang="en">is actor</rdfs:label>
        <skos:altLabel xml:lang="en">Is actor</skos:altLabel>
        <skos:altLabel xml:lang="de">Ist Akteur</skos:altLabel>
    </owl:ObjectProperty>
    


    <!-- &acdh;isAppliedMethod -->

    <owl:ObjectProperty rdf:about="&acdh;isAppliedMethod">
        <rdfs:subPropertyOf rdf:resource="http://www.w3.org/2002/07/owl#topObjectProperty"/>
        <rdfs:domain rdf:resource="&acdh;Concept"/>
        <rdfs:comment xml:lang="en">The methodology (A) applied in creation or curation of the resource or in the project (B) (cf. DataCite: descriptionType methods) </rdfs:comment>
        <rdfs:label xml:lang="en">is applied method</rdfs:label>
        <skos:altLabel xml:lang="en">Is method applied in</skos:altLabel>
        <skos:altLabel xml:lang="de">Ist Methode angewendet in</skos:altLabel>
    </owl:ObjectProperty>
    


    <!-- &acdh;isAuthor -->

    <owl:ObjectProperty rdf:about="&acdh;isAuthor">
        <rdfs:subPropertyOf rdf:resource="&acdh;isCreator"/>
        <rdfs:domain rdf:resource="&acdh;Agent"/>
        <rdfs:range rdf:resource="&acdh;RepoObject"/>
        <rdfs:comment xml:lang="en">Author of resource, who will appear in the citation of it. (??) Has to be distinguished more clearly from creator.</rdfs:comment>
        <rdfs:label xml:lang="en">is author</rdfs:label>
        <skos:altLabel xml:lang="en">Author</skos:altLabel>
        <skos:altLabel xml:lang="de">Verfasser</skos:altLabel>
    </owl:ObjectProperty>
    


    <!-- &acdh;isCategory -->

    <owl:ObjectProperty rdf:about="&acdh;isCategory">
        <rdfs:subPropertyOf rdf:resource="http://www.w3.org/2002/07/owl#topObjectProperty"/>
        <rdfs:domain rdf:resource="&acdh;Concept"/>
        <rdfs:range rdf:resource="&acdh;RepoObject"/>
        <rdfs:comment xml:lang="en">Type of resource, e. g. corpus. Choose from list. Can be refined with description, format, extent, etc.</rdfs:comment>
        <rdfs:comment xml:lang="en">[just for resource type, with controlled vocabulary]</rdfs:comment>
        <rdfs:label xml:lang="en">is category</rdfs:label>
        <skos:altLabel xml:lang="en">Categorises</skos:altLabel>
        <skos:altLabel xml:lang="de">Kategorisiert</skos:altLabel>
    </owl:ObjectProperty>
    


    <!-- &acdh;isCitedBy -->

    <owl:ObjectProperty rdf:about="&acdh;isCitedBy">
        <rdfs:subPropertyOf rdf:resource="&acdh;relation"/>
        <rdfs:domain rdf:resource="&acdh;RepoObject"/>
        <rdfs:range rdf:resource="&acdh;RepoObject"/>
        <rdfs:comment xml:lang="en">Indicates that B includes A in a citation.</rdfs:comment>
        <rdfs:label xml:lang="en">is cited by</rdfs:label>
        <skos:altLabel xml:lang="en">Is cited by</skos:altLabel>
        <skos:altLabel xml:lang="de">Wird zitiert von</skos:altLabel>
    </owl:ObjectProperty>
    


    <!-- &acdh;isCompiledBy -->

    <owl:ObjectProperty rdf:about="&acdh;isCompiledBy">
        <rdfs:subPropertyOf rdf:resource="&acdh;relation"/>
        <rdfs:domain rdf:resource="&acdh;RepoObject"/>
        <rdfs:range rdf:resource="&acdh;RepoObject"/>
        <rdfs:comment xml:lang="en">Indicates B is used to compile or create A.</rdfs:comment>
        <rdfs:label xml:lang="en">is compiled by</rdfs:label>
        <skos:altLabel xml:lang="en">Is compiled by</skos:altLabel>
        <skos:altLabel xml:lang="de">Wird zusammengestellt von</skos:altLabel>
    </owl:ObjectProperty>
    


    <!-- &acdh;isContact -->

    <owl:ObjectProperty rdf:about="&acdh;isContact">
        <rdfs:subPropertyOf rdf:resource="&acdh;isContributor"/>
        <rdfs:domain rdf:resource="&acdh;Agent"/>
        <rdfs:comment xml:lang="en">Person or Organisation that can be contacted regarding information about a Resource or a Project.</rdfs:comment>
        <rdfs:comment xml:lang="en">Person with knowledge of how to access, troubleshoot, or otherwise field issues related to the resource. (DataCite: ContactPerson)</rdfs:comment>
        <rdfs:label xml:lang="en">is contact</rdfs:label>
        <skos:altLabel xml:lang="en">Is contact</skos:altLabel>
        <skos:altLabel xml:lang="de">Ist Kontakt</skos:altLabel>
    </owl:ObjectProperty>
    


    <!-- &acdh;isContinuedBy -->

    <owl:ObjectProperty rdf:about="&acdh;isContinuedBy">
        <rdfs:subPropertyOf rdf:resource="&acdh;relation"/>
        <rdfs:domain rdf:resource="&acdh;RepoObject"/>
        <rdfs:range rdf:resource="&acdh;RepoObject"/>
        <rdfs:comment xml:lang="en">Indicates A is continued by the work B.</rdfs:comment>
        <rdfs:label xml:lang="en">is continued by</rdfs:label>
        <skos:altLabel xml:lang="en">Is continued by</skos:altLabel>
        <skos:altLabel xml:lang="de">Wird fortgesetzt durch</skos:altLabel>
    </owl:ObjectProperty>
    


    <!-- &acdh;isContributor -->

    <owl:ObjectProperty rdf:about="&acdh;isContributor">
        <rdfs:subPropertyOf rdf:resource="http://www.w3.org/2002/07/owl#topObjectProperty"/>
        <rdfs:domain rdf:resource="&acdh;Agent"/>
        <rdfs:comment xml:lang="en"></rdfs:comment>
        <rdfs:comment xml:lang="en">Agent (person, group, organisation) (A) who was actively involved in creating/curating/editing a Resource, a Collection or in a Project (B). Any person or institution making a significant contribution to the development and/or maintenance of the resource, but whose contribution does not “fit” to another already defined role. (cf. DataCite: Other)
This is a generic property. Use one of the more specific sub-properties where possible.</rdfs:comment>
        <rdfs:label xml:lang="en">is contributor</rdfs:label>
        <skos:altLabel xml:lang="en">Contributed to</skos:altLabel>
        <skos:altLabel xml:lang="de">Hat beigetragen zu</skos:altLabel>
    </owl:ObjectProperty>
    


    <!-- &acdh;isCoverage -->

    <owl:ObjectProperty rdf:about="&acdh;isCoverage">
        <rdfs:subPropertyOf rdf:resource="http://www.w3.org/2002/07/owl#topObjectProperty"/>
        <rdfs:domain rdf:resource="&acdh;Concept"/>
        <rdfs:comment xml:lang="en">Description of coverage of content of resource, e.g. spatially and temporally. (??)</rdfs:comment>
        <rdfs:label xml:lang="en">is coverage</rdfs:label>
        <skos:altLabel xml:lang="en">Is covered in</skos:altLabel>
        <skos:altLabel xml:lang="de">Ist abgedeckt in</skos:altLabel>
    </owl:ObjectProperty>
    


    <!-- &acdh;isCreator -->

    <owl:ObjectProperty rdf:about="&acdh;isCreator">
        <rdfs:subPropertyOf rdf:resource="&acdh;isContributor"/>
        <rdfs:domain rdf:resource="&acdh;Agent"/>
        <rdfs:range rdf:resource="&acdh;RepoObject"/>
        <rdfs:comment xml:lang="en">Person involved in the creation of a resource.</rdfs:comment>
        <rdfs:label xml:lang="en">is creator</rdfs:label>
        <skos:altLabel xml:lang="en">Is creator</skos:altLabel>
        <skos:altLabel xml:lang="de">Ist Ersteller</skos:altLabel>
    </owl:ObjectProperty>
    


    <!-- &acdh;isCurator -->

    <owl:ObjectProperty rdf:about="&acdh;isCurator">
        <rdfs:subPropertyOf rdf:resource="&acdh;isContributor"/>
        <rdfs:domain rdf:resource="&acdh;Agent"/>
        <rdfs:range rdf:resource="&acdh;RepoObject"/>
        <rdfs:comment xml:lang="en">Person tasked with reviewing, enhancing, cleaning, or standardizing metadata and the associated data submitted for storage, use, and maintenance within a data centre or repository. (DataCite: DataCurator)</rdfs:comment>
        <rdfs:label xml:lang="en">is curator</rdfs:label>
        <skos:altLabel xml:lang="en">Is data curator</skos:altLabel>
        <skos:altLabel xml:lang="de">Ist Datenkurator</skos:altLabel>
    </owl:ObjectProperty>
    


    <!-- &acdh;isDepositor -->

    <owl:ObjectProperty rdf:about="&acdh;isDepositor">
        <rdfs:subPropertyOf rdf:resource="&acdh;isContributor"/>
        <rdfs:domain rdf:resource="&acdh;Agent"/>
        <rdfs:range rdf:resource="&acdh;RepoObject"/>
        <rdfs:comment xml:lang="en">Person or organisation (A) responsible for submitting a Resource or Collection (B) for hosting to the repository.</rdfs:comment>
        <rdfs:label xml:lang="en">is depositor</rdfs:label>
        <skos:altLabel xml:lang="en">Is depositor</skos:altLabel>
        <skos:altLabel xml:lang="de">Ist Datengeber (hat eingereicht)</skos:altLabel>
    </owl:ObjectProperty>
    


    <!-- &acdh;isDerivedFrom -->

    <owl:ObjectProperty rdf:about="&acdh;isDerivedFrom">
        <rdfs:subPropertyOf rdf:resource="&acdh;relation"/>
        <owl:inverseOf rdf:resource="&acdh;isOriginalFormOf"/>
        <rdfs:domain rdf:resource="&acdh;RepoObject"/>
        <rdfs:range rdf:resource="&acdh;RepoObject"/>
        <rdfs:comment xml:lang="en">Indicates B is a source upon which A is based, e. g. format dng is derived by conversion from format nef.</rdfs:comment>
        <rdfs:label xml:lang="en">is derived from</rdfs:label>
        <skos:altLabel xml:lang="en">Is derived from</skos:altLabel>
        <skos:altLabel xml:lang="de">Ist abgeleitet von</skos:altLabel>
    </owl:ObjectProperty>
    


    <!-- &acdh;isDerivedPublication -->

    <owl:ObjectProperty rdf:about="&acdh;isDerivedPublication">
        <rdfs:subPropertyOf rdf:resource="&acdh;relation"/>
        <rdfs:domain rdf:resource="&acdh;Publication"/>
        <rdfs:comment xml:lang="en">A publication (A) related to a Project, Collection or Resource (B).</rdfs:comment>
        <rdfs:label xml:lang="en">is derived publication</rdfs:label>
        <skos:altLabel xml:lang="en">Is derived publication</skos:altLabel>
        <skos:altLabel xml:lang="de">Ist abgeleitete Publikation</skos:altLabel>
    </owl:ObjectProperty>
    


    <!-- &acdh;isDocumentedBy -->

    <owl:ObjectProperty rdf:about="&acdh;isDocumentedBy">
        <rdfs:subPropertyOf rdf:resource="&acdh;relation"/>
        <rdfs:domain rdf:resource="&acdh;RepoObject"/>
        <rdfs:range rdf:resource="&acdh;RepoObject"/>
        <rdfs:comment xml:lang="en">Indicates B is documentation about/ explaining A.</rdfs:comment>
        <rdfs:label xml:lang="en">is documented by</rdfs:label>
        <skos:altLabel xml:lang="en">Is documented by</skos:altLabel>
        <skos:altLabel xml:lang="de">Ist dokumentiert durch</skos:altLabel>
    </owl:ObjectProperty>
    


    <!-- &acdh;isEditor -->

    <owl:ObjectProperty rdf:about="&acdh;isEditor">
        <rdfs:subPropertyOf rdf:resource="&acdh;isContributor"/>
        <rdfs:domain rdf:resource="&acdh;Agent"/>
        <rdfs:range rdf:resource="&acdh;RepoObject"/>
        <rdfs:comment xml:lang="en">A person who oversees the details related to the publication format of the resource. (DataCite: Editor)</rdfs:comment>
        <rdfs:label xml:lang="en">is editor</rdfs:label>
        <skos:altLabel xml:lang="en">Is editor</skos:altLabel>
        <skos:altLabel xml:lang="de">Ist Herausgeber</skos:altLabel>
    </owl:ObjectProperty>
    


    <!-- &acdh;isFormat -->

    <owl:ObjectProperty rdf:about="&acdh;isFormat">
        <rdfs:subPropertyOf rdf:resource="http://www.w3.org/2002/07/owl#topObjectProperty"/>
        <rdfs:comment xml:lang="en">Format of resource. Indicated as MIME type.</rdfs:comment>
        <rdfs:label xml:lang="en">is format</rdfs:label>
        <skos:altLabel xml:lang="en">Is format</skos:altLabel>
        <skos:altLabel xml:lang="de">Ist Format</skos:altLabel>
    </owl:ObjectProperty>
    


    <!-- &acdh;isFunder -->

    <owl:ObjectProperty rdf:about="&acdh;isFunder">
        <rdfs:subPropertyOf rdf:resource="&acdh;isContributor"/>
        <rdfs:domain rdf:resource="&acdh;Agent"/>
        <rdfs:range rdf:resource="&acdh;Project"/>
        <rdfs:comment xml:lang="en">Person or Organisation which provided funding for the project.</rdfs:comment>
        <rdfs:comment xml:lang="en">Person or organisation that issued a contract or under the auspices of which a work has been written, printed, published, developed, etc. (DataCite: Sponsor)</rdfs:comment>
        <rdfs:label xml:lang="en">is funder</rdfs:label>
        <skos:altLabel xml:lang="de">Hat gefördert</skos:altLabel>
        <skos:altLabel xml:lang="en">Is funder</skos:altLabel>
    </owl:ObjectProperty>
    


    <!-- &acdh;isHosting -->

    <owl:ObjectProperty rdf:about="&acdh;isHosting">
        <rdfs:subPropertyOf rdf:resource="&acdh;isContributor"/>
        <rdfs:domain rdf:resource="&acdh;Agent"/>
        <rdfs:range rdf:resource="&acdh;RepoObject"/>
        <rdfs:comment xml:lang="en">Institution (A) responsible for preservation of a resource (B).</rdfs:comment>
        <rdfs:comment xml:lang="en">Typically, the organisation allowing the resource to be available on the internet through the provision of its hardware/software/operating support. (DataCite: HostingInstitution) </rdfs:comment>
        <rdfs:label xml:lang="en">is hosting</rdfs:label>
        <skos:altLabel xml:lang="de">Erhält und stellt bereit</skos:altLabel>
        <skos:altLabel xml:lang="en">Is hosting</skos:altLabel>
    </owl:ObjectProperty>
    


    <!-- &acdh;isIdenticalTo -->

    <owl:ObjectProperty rdf:about="&acdh;isIdenticalTo">
        <rdfs:subPropertyOf rdf:resource="&acdh;relation"/>
        <rdf:type rdf:resource="http://www.w3.org/2002/07/owl#SymmetricProperty"/>
        <rdfs:domain rdf:resource="&acdh;RepoObject"/>
        <rdfs:range rdf:resource="&acdh;RepoObject"/>
        <rdfs:comment xml:lang="en">Indicates that A is identical to B, for use when there is a need to register two separate instances of the same resource.</rdfs:comment>
        <rdfs:label xml:lang="en">is identical to</rdfs:label>
        <skos:altLabel xml:lang="en">Is identical to</skos:altLabel>
        <skos:altLabel xml:lang="de">Ist identisch mit</skos:altLabel>
    </owl:ObjectProperty>
    


    <!-- &acdh;isLicense -->

    <owl:ObjectProperty rdf:about="&acdh;isLicense">
        <rdfs:subPropertyOf rdf:resource="http://www.w3.org/2002/07/owl#topObjectProperty"/>
        <rdfs:comment xml:lang="en">Denotes the license attached to an object.</rdfs:comment>
        <rdfs:comment>[Martina: rename to isLicense]</rdfs:comment>
        <rdfs:label xml:lang="en">is license</rdfs:label>
        <skos:altLabel xml:lang="en">Licensed</skos:altLabel>
        <skos:altLabel xml:lang="de">Lizensiert durch</skos:altLabel>
    </owl:ObjectProperty>
    


    <!-- &acdh;isLicensor -->

    <owl:ObjectProperty rdf:about="&acdh;isLicensor">
        <rdfs:subPropertyOf rdf:resource="&acdh;isContributor"/>
        <rdfs:domain rdf:resource="&acdh;Agent"/>
        <rdfs:range rdf:resource="&acdh;RepoObject"/>
        <rdfs:comment xml:lang="en">Person or Organisation (A) responsible for choosing a license for the Collection or Resource (B).</rdfs:comment>
        <rdfs:label xml:lang="en">is licensor</rdfs:label>
        <skos:altLabel xml:lang="en">Is licensor</skos:altLabel>
        <skos:altLabel xml:lang="de">Ist Lizenzgeber</skos:altLabel>
    </owl:ObjectProperty>
    


    <!-- &acdh;isLifeCycleStatus -->

    <owl:ObjectProperty rdf:about="&acdh;isLifeCycleStatus">
        <rdfs:subPropertyOf rdf:resource="http://www.w3.org/2002/07/owl#topObjectProperty"/>
        <rdfs:comment xml:lang="en">Is the Project, Collection or Resource still in the making or completed? Should be a controlled list.  A verbose description can be added with acdh:hasCompleteness.</rdfs:comment>
        <rdfs:label xml:lang="en">is life cycle status</rdfs:label>
        <skos:altLabel xml:lang="en">Is life cycle status of</skos:altLabel>
        <skos:altLabel xml:lang="de">Ist Lebenszyklusstatus von</skos:altLabel>
    </owl:ObjectProperty>
    


    <!-- &acdh;isMember -->

    <owl:ObjectProperty rdf:about="&acdh;isMember">
        <rdfs:subPropertyOf rdf:resource="http://www.w3.org/2002/07/owl#topObjectProperty"/>
        <rdfs:range rdf:resource="&acdh;Organisation"/>
        <rdfs:comment xml:lang="en">Used to link a Person to an Organisation or an Organisation (e.g. department) to another Organisation (institution)</rdfs:comment>
        <rdfs:label xml:lang="en">is member</rdfs:label>
        <skos:altLabel xml:lang="en">Is member of</skos:altLabel>
        <skos:altLabel xml:lang="de">Ist Mitglied von</skos:altLabel>
    </owl:ObjectProperty>
    


    <!-- &acdh;isMetadataCreator -->

    <owl:ObjectProperty rdf:about="&acdh;isMetadataCreator">
        <rdfs:subPropertyOf rdf:resource="&acdh;isContributor"/>
        <rdfs:domain rdf:resource="&acdh;Agent"/>
        <rdfs:range rdf:resource="&acdh;RepoObject"/>
        <rdfs:comment xml:lang="en">Person responsible for creating metadata.</rdfs:comment>
        <rdfs:label xml:lang="en">is metadata creator</rdfs:label>
        <skos:altLabel xml:lang="en">Created metadata</skos:altLabel>
        <skos:altLabel xml:lang="de">Hat Metadaten erstellt</skos:altLabel>
    </owl:ObjectProperty>
    


    <!-- &acdh;isMetadataFor -->

    <owl:ObjectProperty rdf:about="&acdh;isMetadataFor">
        <rdfs:subPropertyOf rdf:resource="&acdh;relation"/>
        <rdfs:domain rdf:resource="&acdh;Metadata"/>
        <rdfs:range rdf:resource="&acdh;RepoObject"/>
        <rdfs:comment xml:lang="en">Indicates additional metadata A for a resource B.</rdfs:comment>
        <rdfs:label xml:lang="en">is metadata for</rdfs:label>
        <skos:altLabel xml:lang="de">Enthält Metadaten für</skos:altLabel>
        <skos:altLabel xml:lang="en">Is metadata for</skos:altLabel>
    </owl:ObjectProperty>
    


    <!-- &acdh;isNewVersionOf -->

    <owl:ObjectProperty rdf:about="&acdh;isNewVersionOf">
        <rdfs:subPropertyOf rdf:resource="&acdh;relation"/>
        <owl:inverseOf rdf:resource="&acdh;isPreviousVersionOf"/>
        <rdfs:domain rdf:resource="&acdh;RepoObject"/>
        <rdfs:range rdf:resource="&acdh;RepoObject"/>
        <rdfs:comment xml:lang="en">Indicates A is a new edition of B, where the new edition has been modified or updated.</rdfs:comment>
        <rdfs:label xml:lang="en">is new version of</rdfs:label>
        <skos:altLabel xml:lang="en">Is new version of</skos:altLabel>
        <skos:altLabel xml:lang="de">Ist neue Version von</skos:altLabel>
    </owl:ObjectProperty>
    


    <!-- &acdh;isOriginalFormOf -->

    <owl:ObjectProperty rdf:about="&acdh;isOriginalFormOf">
        <rdfs:subPropertyOf rdf:resource="&acdh;relation"/>
        <owl:inverseOf rdf:resource="&acdh;isVariantFormOf"/>
        <rdfs:domain rdf:resource="&acdh;RepoObject"/>
        <rdfs:range rdf:resource="&acdh;RepoObject"/>
        <rdfs:comment xml:lang="en">Indicates A is the original form of B, e. g. format nef is orignial of converted format dng.</rdfs:comment>
        <rdfs:label xml:lang="en">is original form of</rdfs:label>
        <skos:altLabel xml:lang="en">Is original form of</skos:altLabel>
        <skos:altLabel xml:lang="de">Originale Form von</skos:altLabel>
    </owl:ObjectProperty>
    


    <!-- &acdh;isOwner -->

    <owl:ObjectProperty rdf:about="&acdh;isOwner">
        <rdfs:subPropertyOf rdf:resource="&acdh;isContributor"/>
        <rdfs:domain rdf:resource="&acdh;Agent"/>
        <rdfs:range rdf:resource="&acdh;RepoObject"/>
        <rdfs:comment xml:lang="en">A Person or Organisation (A) owning a Collection or Resource (B).</rdfs:comment>
        <rdfs:label xml:lang="en">is owner</rdfs:label>
        <skos:altLabel xml:lang="en">Is owner</skos:altLabel>
        <skos:altLabel xml:lang="de">Ist Besitzer von</skos:altLabel>
    </owl:ObjectProperty>
    


    <!-- &acdh;isPartOf -->

    <owl:ObjectProperty rdf:about="&acdh;isPartOf">
        <rdfs:subPropertyOf rdf:resource="&acdh;relation"/>
        <rdfs:domain rdf:resource="&acdh;RepoObject"/>
        <rdfs:range rdf:resource="&acdh;Collection"/>
        <rdfs:comment xml:lang="en">Indicates A is a part of aggregate B, e. g. elements of a series, items of a collection.</rdfs:comment>
        <rdfs:label xml:lang="en">is part of</rdfs:label>
        <skos:altLabel xml:lang="en">Is part of</skos:altLabel>
        <skos:altLabel xml:lang="de">Ist Teil von</skos:altLabel>
    </owl:ObjectProperty>
    


    <!-- &acdh;isPreviousVersionOf -->

    <owl:ObjectProperty rdf:about="&acdh;isPreviousVersionOf">
        <rdfs:subPropertyOf rdf:resource="&acdh;relation"/>
        <rdfs:domain rdf:resource="&acdh;RepoObject"/>
        <rdfs:range rdf:resource="&acdh;RepoObject"/>
        <rdfs:comment xml:lang="en">Indicates A is a previous edition of B.</rdfs:comment>
        <rdfs:label xml:lang="en">is previous version of</rdfs:label>
        <skos:altLabel xml:lang="en">Is previous version of</skos:altLabel>
        <skos:altLabel xml:lang="de">Ist vorhergehende Version von</skos:altLabel>
    </owl:ObjectProperty>
    


    <!-- &acdh;isPrincipalInvestigator -->

    <owl:ObjectProperty rdf:about="&acdh;isPrincipalInvestigator">
        <rdfs:subPropertyOf rdf:resource="&acdh;isContributor"/>
        <rdfs:domain rdf:resource="&acdh;Agent"/>
        <rdfs:range rdf:resource="&acdh;Project"/>
        <rdfs:comment xml:lang="en">Person officially designated as head of project team or subproject team instrumental in the work necessary to development of the resource. (DataCite: ProjectLeader)</rdfs:comment>
        <rdfs:label xml:lang="en">is principal investigator</rdfs:label>
        <skos:altLabel xml:lang="en">Is principal investigator</skos:altLabel>
        <skos:altLabel xml:lang="de">Ist Primärforscher</skos:altLabel>
    </owl:ObjectProperty>
    


    <!-- &acdh;isPublicationPlace -->

    <owl:ObjectProperty rdf:about="&acdh;isPublicationPlace">
        <rdfs:comment xml:lang="en">Connects a Publication with a Place, where it was published.</rdfs:comment>
        <rdfs:label xml:lang="en">has publication place</rdfs:label>
        <skos:altLabel xml:lang="en">Publication place</skos:altLabel>
        <skos:altLabel xml:lang="de">Veröffentlichungsort</skos:altLabel>
    </owl:ObjectProperty>
    


    <!-- &acdh;isReferencedBy -->

    <owl:ObjectProperty rdf:about="&acdh;isReferencedBy">
        <rdfs:subPropertyOf rdf:resource="&acdh;relation"/>
        <owl:inverseOf rdf:resource="&acdh;references"/>
        <rdfs:domain rdf:resource="&acdh;RepoObject"/>
        <rdfs:range rdf:resource="&acdh;RepoObject"/>
        <rdfs:comment xml:lang="en">Indicates A is used as a source of information by B.</rdfs:comment>
        <rdfs:label xml:lang="en">is referenced by</rdfs:label>
        <skos:altLabel xml:lang="en">Is referenced by</skos:altLabel>
        <skos:altLabel xml:lang="de">Wird referenziert von</skos:altLabel>
    </owl:ObjectProperty>
    


    <!-- &acdh;isRelatedDiscipline -->

    <owl:ObjectProperty rdf:about="&acdh;isRelatedDiscipline">
        <rdfs:subPropertyOf rdf:resource="http://www.w3.org/2002/07/owl#topObjectProperty"/>
        <rdfs:domain rdf:resource="&acdh;Concept"/>
        <rdfs:comment xml:lang="en">Discipline of Project, Collection or Resource. Can be used for search.</rdfs:comment>
        <rdfs:comment>[Martina: should this be a sub of relation?]</rdfs:comment>
        <rdfs:label xml:lang="en">is related discipline</rdfs:label>
        <skos:altLabel xml:lang="en">Is related discipline of</skos:altLabel>
        <skos:altLabel xml:lang="de">Ist zugehörige Disziplin von</skos:altLabel>
    </owl:ObjectProperty>
    


    <!-- &acdh;isReviewedBy -->

    <owl:ObjectProperty rdf:about="&acdh;isReviewedBy">
        <rdfs:subPropertyOf rdf:resource="&acdh;relation"/>
        <owl:inverseOf rdf:resource="&acdh;reviews"/>
        <rdfs:domain rdf:resource="&acdh;RepoObject"/>
        <rdfs:range rdf:resource="&acdh;RepoObject"/>
        <rdfs:comment xml:lang="en">Indicates that B is review of A.</rdfs:comment>
        <rdfs:label xml:lang="en">is reviewed by</rdfs:label>
        <skos:altLabel xml:lang="en">Is reviewed by</skos:altLabel>
        <skos:altLabel xml:lang="de">Wird reviewed durch</skos:altLabel>
    </owl:ObjectProperty>
    


    <!-- &acdh;isRightsHolder -->

    <owl:ObjectProperty rdf:about="&acdh;isRightsHolder">
        <rdfs:subPropertyOf rdf:resource="&acdh;isContributor"/>
        <rdfs:domain rdf:resource="&acdh;Agent"/>
        <rdfs:range rdf:resource="&acdh;RepoObject"/>
        <rdfs:comment xml:lang="en">Person or institution owning or managing property rights, including intellectual property rights over the resource. (DataCite: RightsHolder)</rdfs:comment>
        <rdfs:label xml:lang="en">is rights holder</rdfs:label>
        <skos:altLabel xml:lang="en">Is rights holder</skos:altLabel>
        <skos:altLabel xml:lang="de">Ist Rechteinhaber</skos:altLabel>
    </owl:ObjectProperty>
    


    <!-- &acdh;isSchema -->

    <owl:ObjectProperty rdf:about="&acdh;isSchema">
        <rdfs:subPropertyOf rdf:resource="http://www.w3.org/2002/07/owl#topObjectProperty"/>
        <rdfs:domain rdf:resource="&acdh;Resource"/>
        <rdfs:range rdf:resource="&acdh;Resource"/>
        <rdfs:comment xml:lang="en">Reference to a resource (B) adhering to the schema (A)</rdfs:comment>
        <rdfs:label xml:lang="en">is schema</rdfs:label>
        <skos:altLabel xml:lang="en">Is schema of</skos:altLabel>
        <skos:altLabel xml:lang="de">Ist Schema von</skos:altLabel>
    </owl:ObjectProperty>
    


    <!-- &acdh;isSourceOf -->

    <owl:ObjectProperty rdf:about="&acdh;isSourceOf">
        <rdfs:subPropertyOf rdf:resource="&acdh;relation"/>
        <rdfs:domain rdf:resource="&acdh;RepoObject"/>
        <rdfs:range rdf:resource="&acdh;RepoObject"/>
        <rdfs:comment xml:lang="en">Indicates A is a source upon which B is based.</rdfs:comment>
        <rdfs:label xml:lang="en">is source of</rdfs:label>
        <skos:altLabel xml:lang="en">Is source of</skos:altLabel>
        <skos:altLabel xml:lang="de">Ist Quelle von</skos:altLabel>
    </owl:ObjectProperty>
    


    <!-- &acdh;isSpatialCoverage -->

    <owl:ObjectProperty rdf:about="&acdh;isSpatialCoverage">
        <rdfs:subPropertyOf rdf:resource="&acdh;isCoverage"/>
        <rdfs:domain rdf:resource="&acdh;Place"/>
        <rdfs:comment xml:lang="en">A  place, geographic location (A) covered/mentioned in a Project, Collection or Resource (B); e.g. &apos;Pannonia&apos; as a location for data from archaeological excavations or &apos;Austria&apos; as a originating place for a collection of digitised newspapers.</rdfs:comment>
        <rdfs:label xml:lang="en">is spatial coverage</rdfs:label>
        <skos:altLabel xml:lang="de">Geografisch behandelt in</skos:altLabel>
        <skos:altLabel xml:lang="en">Spatially covered in</skos:altLabel>
    </owl:ObjectProperty>
    


    <!-- &acdh;isSubject -->

    <owl:ObjectProperty rdf:about="&acdh;isSubject">
        <rdfs:subPropertyOf rdf:resource="&acdh;isCoverage"/>
        <rdfs:domain rdf:resource="&acdh;Concept"/>
        <rdfs:comment xml:lang="en">Subject of Project, Collection or Resource. Can be used as keywords for search.</rdfs:comment>
        <rdfs:label xml:lang="en">is subject</rdfs:label>
        <skos:altLabel xml:lang="en">Is subject of</skos:altLabel>
        <skos:altLabel xml:lang="de">Ist Gegenstand von</skos:altLabel>
    </owl:ObjectProperty>
    


    <!-- &acdh;isSupplementTo -->

    <owl:ObjectProperty rdf:about="&acdh;isSupplementTo">
        <rdfs:subPropertyOf rdf:resource="&acdh;relation"/>
        <owl:inverseOf rdf:resource="&acdh;isSupplementedBy"/>
        <rdfs:domain rdf:resource="&acdh;RepoObject"/>
        <rdfs:range rdf:resource="&acdh;RepoObject"/>
        <rdfs:comment xml:lang="en">Indicates that A is a supplement to B.</rdfs:comment>
        <rdfs:label xml:lang="en">is supplement to</rdfs:label>
        <skos:altLabel xml:lang="en">Is supplement to</skos:altLabel>
        <skos:altLabel xml:lang="de">Ist Ergänzung zu</skos:altLabel>
    </owl:ObjectProperty>
    


    <!-- &acdh;isSupplementedBy -->

    <owl:ObjectProperty rdf:about="&acdh;isSupplementedBy">
        <rdfs:subPropertyOf rdf:resource="&acdh;relation"/>
        <rdfs:domain rdf:resource="&acdh;RepoObject"/>
        <rdfs:range rdf:resource="&acdh;RepoObject"/>
        <rdfs:comment xml:lang="en">Indicates that B is a supplement to A.</rdfs:comment>
        <rdfs:label xml:lang="en">is supplemented by</rdfs:label>
        <skos:altLabel xml:lang="en">Is supplemented by</skos:altLabel>
        <skos:altLabel xml:lang="de">Wird ergänzt von</skos:altLabel>
    </owl:ObjectProperty>
    


    <!-- &acdh;isTitleImageOf -->

    <owl:ObjectProperty rdf:about="&acdh;isTitleImageOf">
        <rdfs:subPropertyOf rdf:resource="&acdh;relation"/>
        <rdfs:domain rdf:resource="&acdh;Image"/>
        <rdfs:range rdf:resource="&acdh;RepoObject"/>
        <rdfs:comment xml:lang="en">Title image or logo of Organisation, Project, Collection or Resource used for presentation.</rdfs:comment>
        <rdfs:label xml:lang="en">is title image of</rdfs:label>
        <skos:altLabel xml:lang="en">Is title image of</skos:altLabel>
        <skos:altLabel xml:lang="de">Ist Titelbild von</skos:altLabel>
    </owl:ObjectProperty>
    


    <!-- &acdh;isTransferMethod -->

    <owl:ObjectProperty rdf:about="&acdh;isTransferMethod">
        <rdfs:subPropertyOf rdf:resource="http://www.w3.org/2002/07/owl#topObjectProperty"/>
        <rdfs:domain rdf:resource="&acdh;Concept"/>
        <rdfs:range rdf:resource="&acdh;RepoObject"/>
        <rdfs:comment xml:lang="en">Method used to transfer resources from depositor to repository.</rdfs:comment>
        <rdfs:label xml:lang="en">is transfer method</rdfs:label>
        <skos:altLabel xml:lang="en">Is transfer method</skos:altLabel>
        <skos:altLabel xml:lang="de">Ist Transfermethode</skos:altLabel>
    </owl:ObjectProperty>
    


    <!-- &acdh;isVariantFormOf -->

    <owl:ObjectProperty rdf:about="&acdh;isVariantFormOf">
        <rdfs:subPropertyOf rdf:resource="&acdh;relation"/>
        <rdfs:domain rdf:resource="&acdh;RepoObject"/>
        <rdfs:range rdf:resource="&acdh;RepoObject"/>
        <rdfs:comment xml:lang="en">Indicates A is a variant or different form of B, e.g. calculated or calibrated from or different packaging</rdfs:comment>
        <rdfs:label xml:lang="en">is variant form of</rdfs:label>
        <skos:altLabel xml:lang="en">Is variant form of</skos:altLabel>
        <skos:altLabel xml:lang="de">Ist Variante von</skos:altLabel>
    </owl:ObjectProperty>
    


    <!-- &acdh;references -->

    <owl:ObjectProperty rdf:about="&acdh;references">
        <rdfs:subPropertyOf rdf:resource="&acdh;relation"/>
        <rdfs:domain rdf:resource="&acdh;RepoObject"/>
        <rdfs:range rdf:resource="&acdh;RepoObject"/>
        <rdfs:comment xml:lang="en">Indicates B is used as a source of information for A.</rdfs:comment>
        <rdfs:label xml:lang="en">references</rdfs:label>
        <skos:altLabel xml:lang="en">References</skos:altLabel>
        <skos:altLabel xml:lang="de">Referenziert</skos:altLabel>
    </owl:ObjectProperty>
    


    <!-- &acdh;relation -->

    <owl:ObjectProperty rdf:about="&acdh;relation">
        <rdfs:subPropertyOf rdf:resource="http://www.w3.org/2002/07/owl#topObjectProperty"/>
        <rdfs:domain rdf:resource="&acdh;RepoObject"/>
        <rdfs:range rdf:resource="&acdh;RepoObject"/>
        <rdfs:comment xml:lang="en">A generic indication of any relation between two resources. Preferably use any of the more specific subproperties.</rdfs:comment>
        <rdfs:label xml:lang="en">relation</rdfs:label>
        <skos:altLabel xml:lang="de">Relation</skos:altLabel>
        <skos:altLabel xml:lang="en">Relation</skos:altLabel>
    </owl:ObjectProperty>
    


    <!-- &acdh;reviews -->

    <owl:ObjectProperty rdf:about="&acdh;reviews">
        <rdfs:subPropertyOf rdf:resource="&acdh;relation"/>
        <rdfs:domain rdf:resource="&acdh;RepoObject"/>
        <rdfs:range rdf:resource="&acdh;RepoObject"/>
        <rdfs:comment xml:lang="en">Indicates that A is a review of B.</rdfs:comment>
        <rdfs:label xml:lang="en">reviews</rdfs:label>
        <skos:altLabel xml:lang="de">Ist ein Review von</skos:altLabel>
        <skos:altLabel xml:lang="en">Reviews</skos:altLabel>
    </owl:ObjectProperty>
    


    <!-- 
    ///////////////////////////////////////////////////////////////////////////////////////
    //
    // Data properties
    //
    ///////////////////////////////////////////////////////////////////////////////////////
     -->

    


    <!-- http://purl.org/dc/elements/1.1/date -->

    <owl:DatatypeProperty rdf:about="http://purl.org/dc/elements/1.1/date">
        <owl:equivalentProperty rdf:resource="&acdh;hasDate"/>
    </owl:DatatypeProperty>
    


    <!-- http://purl.org/dc/elements/1.1/description -->

    <owl:DatatypeProperty rdf:about="http://purl.org/dc/elements/1.1/description">
        <owl:equivalentProperty rdf:resource="&acdh;hasDescription"/>
    </owl:DatatypeProperty>
    


    <!-- http://purl.org/dc/elements/1.1/identifier -->

    <owl:DatatypeProperty rdf:about="http://purl.org/dc/elements/1.1/identifier">
        <owl:equivalentProperty rdf:resource="&acdh;hasIdentifier"/>
        <owl:equivalentProperty rdf:resource="&acdh;hasPid"/>
    </owl:DatatypeProperty>
    


    <!-- http://purl.org/dc/elements/1.1/language -->

    <owl:DatatypeProperty rdf:about="http://purl.org/dc/elements/1.1/language">
        <owl:equivalentProperty rdf:resource="&acdh;language"/>
    </owl:DatatypeProperty>
    


    <!-- http://purl.org/dc/elements/1.1/title -->

    <owl:DatatypeProperty rdf:about="http://purl.org/dc/elements/1.1/title">
        <owl:equivalentProperty rdf:resource="&acdh;hasTitle"/>
    </owl:DatatypeProperty>
    


    <!-- http://vocabs.acdh.oeaw.ac.at#hasFirstName -->

    <owl:DatatypeProperty rdf:about="http://vocabs.acdh.oeaw.ac.at#hasFirstName">
        <rdfs:subPropertyOf rdf:resource="http://www.w3.org/2002/07/owl#topDataProperty"/>
        <rdfs:domain rdf:resource="&acdh;Person"/>
        <rdfs:range rdf:resource="http://www.w3.org/2000/01/rdf-schema#Literal"/>
        <rdfs:comment xml:lang="en">First name of a Person.</rdfs:comment>
        <rdfs:label xml:lang="en">has first name</rdfs:label>
        <skos:altLabel xml:lang="de">First name</skos:altLabel>
        <skos:altLabel xml:lang="en">Vorname</skos:altLabel>
    </owl:DatatypeProperty>
    


    <!-- http://vocabs.acdh.oeaw.ac.at#hasLastName -->

    <owl:DatatypeProperty rdf:about="http://vocabs.acdh.oeaw.ac.at#hasLastName">
        <rdfs:subPropertyOf rdf:resource="http://www.w3.org/2002/07/owl#topDataProperty"/>
        <rdfs:domain rdf:resource="&acdh;Person"/>
        <rdfs:range rdf:resource="http://www.w3.org/2000/01/rdf-schema#Literal"/>
        <rdfs:comment xml:lang="en">Last Name of Person.</rdfs:comment>
        <rdfs:label xml:lang="en">has last name</rdfs:label>
        <skos:altLabel xml:lang="de">Last name</skos:altLabel>
        <skos:altLabel xml:lang="en">Nachname</skos:altLabel>
    </owl:DatatypeProperty>
    


    <!-- &acdh;hasAcceptedDate -->

    <owl:DatatypeProperty rdf:about="&acdh;hasAcceptedDate">
        <rdfs:subPropertyOf rdf:resource="&acdh;hasDate"/>
        <rdfs:domain rdf:resource="&acdh;RepoObject"/>
        <rdfs:range rdf:resource="http://www.w3.org/2001/XMLSchema#date"/>
        <rdfs:comment xml:lang="de">Datum an dem die Ressource angenommen wurde.</rdfs:comment>
        <rdfs:comment xml:lang="en">The date that the publisher accepted the resource into their system.</rdfs:comment>
        <rdfs:label xml:lang="en">has accepted date</rdfs:label>
        <skos:altLabel xml:lang="de">Annahmedatum</skos:altLabel>
        <skos:altLabel xml:lang="en">Date of Acceptance</skos:altLabel>
    </owl:DatatypeProperty>
    


    <!-- &acdh;hasAddress -->

    <owl:DatatypeProperty rdf:about="&acdh;hasAddress">
        <rdfs:range rdf:resource="http://www.w3.org/2000/01/rdf-schema#Literal"/>
        <rdfs:comment xml:lang="en">Adress associated with a Person or Organisation. Use sub-properties to input detailed information like postcode, city and country.</rdfs:comment>
        <rdfs:label xml:lang="en">has address</rdfs:label>
        <skos:altLabel xml:lang="en">Address</skos:altLabel>
        <skos:altLabel xml:lang="de">Adresse</skos:altLabel>
    </owl:DatatypeProperty>
    


    <!-- &acdh;hasAddressLine1 -->

    <owl:DatatypeProperty rdf:about="&acdh;hasAddressLine1">
        <rdfs:subPropertyOf rdf:resource="&acdh;hasAddress"/>
        <rdfs:range rdf:resource="http://www.w3.org/2000/01/rdf-schema#Literal"/>
        <rdfs:comment xml:lang="en">First line of adress associated with a Person or Organisation.</rdfs:comment>
        <rdfs:label xml:lang="en">has address line 1</rdfs:label>
        <skos:altLabel xml:lang="de">Addresszeile 1</skos:altLabel>
        <skos:altLabel xml:lang="en">Adresse Line 1</skos:altLabel>
    </owl:DatatypeProperty>
    


    <!-- &acdh;hasAddressLine2 -->

    <owl:DatatypeProperty rdf:about="&acdh;hasAddressLine2">
        <rdfs:subPropertyOf rdf:resource="&acdh;hasAddress"/>
        <rdfs:range rdf:resource="http://www.w3.org/2000/01/rdf-schema#Literal"/>
        <rdfs:comment xml:lang="en">Second line of adress associated with a Person or Organisation.</rdfs:comment>
        <rdfs:label xml:lang="en">has address line 2</rdfs:label>
        <skos:altLabel xml:lang="de">Addresszeile 2</skos:altLabel>
        <skos:altLabel xml:lang="en">Adresse Line 2</skos:altLabel>
    </owl:DatatypeProperty>
    


    <!-- &acdh;hasAlternativeTitle -->

    <owl:DatatypeProperty rdf:about="&acdh;hasAlternativeTitle">
        <rdfs:range rdf:resource="http://www.w3.org/2000/01/rdf-schema#Literal"/>
        <rdfs:comment xml:lang="en">Alternative title or name of Project, Collection or Resource. Can also be used as alternative name for an organisation.</rdfs:comment>
        <rdfs:label xml:lang="en">has alternative title</rdfs:label>
        <skos:altLabel xml:lang="en">Alternative title</skos:altLabel>
        <skos:altLabel xml:lang="de">Alternativtitel</skos:altLabel>
    </owl:DatatypeProperty>
    


    <!-- &acdh;hasAppliedMethodDescription -->

    <owl:DatatypeProperty rdf:about="&acdh;hasAppliedMethodDescription">
        <rdfs:subPropertyOf rdf:resource="&acdh;hasDescription"/>
        <rdfs:domain rdf:resource="&acdh;RepoObject"/>
        <rdfs:range rdf:resource="http://www.w3.org/2000/01/rdf-schema#Literal"/>
        <rdfs:comment xml:lang="en">Verbose description of the methodology employed in the creation/curation of a resource. (cf. DataCite descriptionType methods). </rdfs:comment>
        <rdfs:label xml:lang="en">has applied method description</rdfs:label>
        <rdfs:seeAlso>acdh:appliedMethod a owl:ObjectProperty</rdfs:seeAlso>
        <skos:altLabel xml:lang="de">Angewandte Methoden</skos:altLabel>
        <skos:altLabel xml:lang="en">Applied Method</skos:altLabel>
    </owl:DatatypeProperty>
    


    <!-- &acdh;hasArrangement -->

    <owl:DatatypeProperty rdf:about="&acdh;hasArrangement">
        <rdfs:subPropertyOf rdf:resource="&acdh;hasDescription"/>
        <rdfs:domain rdf:resource="&acdh;RepoObject"/>
        <rdfs:range rdf:resource="http://www.w3.org/2000/01/rdf-schema#Literal"/>
        <rdfs:comment xml:lang="en">Indicates a logical and coherent overall view of the whole set of objects. Here the description of folder structure, nature of relationship between objects and metadata, etc. are expected. If necessary, diagrams or screenshots from the original system can be included.</rdfs:comment>
        <rdfs:label xml:lang="en">has arrangement</rdfs:label>
        <skos:altLabel xml:lang="en">Description of arrangement</skos:altLabel>
        <skos:altLabel xml:lang="de">Strukturbeschreibung</skos:altLabel>
    </owl:DatatypeProperty>
    


    <!-- &acdh;hasAvailableDate -->

    <owl:DatatypeProperty rdf:about="&acdh;hasAvailableDate">
        <rdfs:subPropertyOf rdf:resource="&acdh;hasDate"/>
        <rdfs:domain rdf:resource="&acdh;RepoObject"/>
        <rdfs:range rdf:resource="http://www.w3.org/2001/XMLSchema#date"/>
        <rdfs:comment xml:lang="de">Datum seit dem die Ressource öffentlich verfügbar ist.</rdfs:comment>
        <rdfs:comment xml:lang="en">The date the resource is made publicly available.</rdfs:comment>
        <rdfs:label xml:lang="en">has available date</rdfs:label>
        <skos:altLabel xml:lang="en">Available since</skos:altLabel>
        <skos:altLabel xml:lang="de">Verfügbar seit</skos:altLabel>
    </owl:DatatypeProperty>
    


    <!-- &acdh;hasBinarySize -->

    <owl:DatatypeProperty rdf:about="&acdh;hasBinarySize">
        <rdfs:subPropertyOf rdf:resource="&acdh;hasDescription"/>
        <rdfs:domain rdf:resource="&acdh;RepoObject"/>
        <rdfs:range rdf:resource="http://www.w3.org/2001/XMLSchema#byte"/>
        <rdfs:comment xml:lang="en">Indicates size in bytes of a Resource or Collection.</rdfs:comment>
        <rdfs:label xml:lang="en">has binary size</rdfs:label>
        <skos:altLabel xml:lang="en">Größe</skos:altLabel>
        <skos:altLabel xml:lang="de">Size</skos:altLabel>
    </owl:DatatypeProperty>
    


    <!-- &acdh;hasCharacterEncoding -->

    <owl:DatatypeProperty rdf:about="&acdh;hasCharacterEncoding">
        <rdfs:subPropertyOf rdf:resource="http://www.w3.org/2002/07/owl#topDataProperty"/>
        <rdfs:domain rdf:resource="&acdh;Resource"/>
        <rdfs:range rdf:resource="http://www.w3.org/2000/01/rdf-schema#Literal"/>
        <rdfs:comment xml:lang="en">Information about character encoding used and also information about nonstandard characters and glyphs used.
Indicate character encoding according to the overview of Character Sets by IANA: https://www.iana.org/assignments/character-sets/character-sets.xhtml</rdfs:comment>
        <rdfs:label xml:lang="en">has character encoding</rdfs:label>
        <skos:altLabel xml:lang="en">Character encoding</skos:altLabel>
        <skos:altLabel xml:lang="de">Zeichenkodierung</skos:altLabel>
    </owl:DatatypeProperty>
    


    <!-- &acdh;hasCity -->

    <owl:DatatypeProperty rdf:about="&acdh;hasCity">
        <rdfs:subPropertyOf rdf:resource="&acdh;hasAddress"/>
        <rdfs:range rdf:resource="http://www.w3.org/2000/01/rdf-schema#Literal"/>
        <rdfs:comment xml:lang="en">City or Town of adress associated with a Person or Organisation.</rdfs:comment>
        <rdfs:label xml:lang="en">has city</rdfs:label>
        <skos:altLabel xml:lang="en">City/Town</skos:altLabel>
        <skos:altLabel xml:lang="de">Stadt</skos:altLabel>
    </owl:DatatypeProperty>
    


    <!-- &acdh;hasCollectedEndDate -->

    <owl:DatatypeProperty rdf:about="&acdh;hasCollectedEndDate">
        <rdfs:subPropertyOf rdf:resource="&acdh;hasDate"/>
        <rdfs:domain rdf:resource="&acdh;RepoObject"/>
        <rdfs:range rdf:resource="http://www.w3.org/2001/XMLSchema#date"/>
        <rdfs:comment xml:lang="de">Datum oder Zeitraum in dem der Inhalt der Ressource zusammengestellt wurde. Enddatum</rdfs:comment>
        <rdfs:comment xml:lang="en">The date or date range in which the resource content was collected. End date.</rdfs:comment>
        <rdfs:label xml:lang="en">has collected end date</rdfs:label>
        <skos:altLabel xml:lang="en">Date of data collection (end)</skos:altLabel>
        <skos:altLabel xml:lang="de">Datum der Zusammenstellung (Ende)</skos:altLabel>
    </owl:DatatypeProperty>
    


    <!-- &acdh;hasCollectedStartDate -->

    <owl:DatatypeProperty rdf:about="&acdh;hasCollectedStartDate">
        <rdfs:subPropertyOf rdf:resource="&acdh;hasDate"/>
        <rdfs:domain rdf:resource="&acdh;RepoObject"/>
        <rdfs:range rdf:resource="http://www.w3.org/2001/XMLSchema#date"/>
        <rdfs:comment xml:lang="de">Datum oder Zeitraum in dem der Inhalt der Ressource zusammengestellt wurde. Startddatum</rdfs:comment>
        <rdfs:comment xml:lang="en">The date or date range in which the resource content was collected. Start date.</rdfs:comment>
        <rdfs:label xml:lang="en">has collected start date</rdfs:label>
        <skos:altLabel xml:lang="en">Date of data collection (start)</skos:altLabel>
        <skos:altLabel xml:lang="de">Datum der Zusammenstellung (Start)</skos:altLabel>
    </owl:DatatypeProperty>
    


    <!-- &acdh;hasCompleteness -->

    <owl:DatatypeProperty rdf:about="&acdh;hasCompleteness">
        <rdfs:subPropertyOf rdf:resource="&acdh;hasDescription"/>
        <rdfs:domain rdf:resource="&acdh;RepoObject"/>
        <rdfs:range rdf:resource="http://www.w3.org/2000/01/rdf-schema#Literal"/>
        <rdfs:comment xml:lang="en">Descriptive statement about how complete the resource is.</rdfs:comment>
        <rdfs:label xml:lang="en">has completeness</rdfs:label>
        <rdfs:seeAlso>acdh:hasLifeCycleStatus</rdfs:seeAlso>
        <skos:altLabel xml:lang="de">Angaben zur Vollständigkeit</skos:altLabel>
        <skos:altLabel xml:lang="en">Completeness statement</skos:altLabel>
    </owl:DatatypeProperty>
    


    <!-- &acdh;hasCopyrightedDate -->

    <owl:DatatypeProperty rdf:about="&acdh;hasCopyrightedDate">
        <rdfs:subPropertyOf rdf:resource="&acdh;hasDate"/>
        <rdfs:domain rdf:resource="&acdh;RepoObject"/>
        <rdfs:range rdf:resource="http://www.w3.org/2001/XMLSchema#date"/>
        <rdfs:comment xml:lang="de">Datum seit dem die Ressource urheberrechtlich geschützt ist, wenn anwendbar.</rdfs:comment>
        <rdfs:comment xml:lang="en">The specific, documented date at which the resource receives a copyrighted status, if applicable.</rdfs:comment>
        <rdfs:label xml:lang="en">has copyrighted date</rdfs:label>
        <skos:altLabel xml:lang="en">Date of Copyright Protection</skos:altLabel>
        <skos:altLabel xml:lang="de">Urheberrechtlich geschützt seit</skos:altLabel>
    </owl:DatatypeProperty>
    


    <!-- &acdh;hasCountry -->

    <owl:DatatypeProperty rdf:about="&acdh;hasCountry">
        <rdfs:subPropertyOf rdf:resource="&acdh;hasAddress"/>
        <rdfs:range rdf:resource="http://www.w3.org/2000/01/rdf-schema#Literal"/>
        <rdfs:comment xml:lang="en">Country of adress associated with a Person or Organisation.</rdfs:comment>
        <rdfs:label xml:lang="en">has country</rdfs:label>
        <skos:altLabel xml:lang="en">Country</skos:altLabel>
        <skos:altLabel xml:lang="de">Land</skos:altLabel>
    </owl:DatatypeProperty>
    


    <!-- &acdh;hasCoverageEndDate -->

    <owl:DatatypeProperty rdf:about="&acdh;hasCoverageEndDate">
        <rdfs:subPropertyOf rdf:resource="&acdh;hasDate"/>
        <rdfs:range rdf:resource="http://www.w3.org/2001/XMLSchema#date"/>
        <rdfs:comment xml:lang="en">End date for temporal coverage, i.e. end of the period a Project, Collection or Resource (A) deals with.</rdfs:comment>
        <rdfs:label xml:lang="en">has coverage end date</rdfs:label>
        <skos:altLabel xml:lang="en">Coverage end date</skos:altLabel>
        <skos:altLabel xml:lang="de">Ende der abgedeckten Zeitperiode</skos:altLabel>
    </owl:DatatypeProperty>
    


    <!-- &acdh;hasCoverageStartDate -->

    <owl:DatatypeProperty rdf:about="&acdh;hasCoverageStartDate">
        <rdfs:subPropertyOf rdf:resource="&acdh;hasDate"/>
        <rdfs:range rdf:resource="http://www.w3.org/2001/XMLSchema#date"/>
        <rdfs:comment xml:lang="en">Start date for temporal coverage (B), i.e. beginning of the period a Project, Collection or Resource (A) deals with.</rdfs:comment>
        <rdfs:label xml:lang="en">has coverage start date</rdfs:label>
        <skos:altLabel xml:lang="de">Anfang der abgedeckten Periode</skos:altLabel>
        <skos:altLabel xml:lang="en">Coverage start date</skos:altLabel>
    </owl:DatatypeProperty>
    


    <!-- &acdh;hasCreatedDate -->

    <owl:DatatypeProperty rdf:about="&acdh;hasCreatedDate">
        <rdfs:subPropertyOf rdf:resource="&acdh;hasDate"/>
        <rdfs:range rdf:resource="http://www.w3.org/2001/XMLSchema#date"/>
        <rdfs:comment xml:lang="de">Datum der Erstellung oder Zusammenstellung der Ressource oder Collection. Wird für die Angabe von einem einzelnen Datum verwendet. Für eine Zeitspanne Eigenschaft &apos;hasCreatedDate&apos; verwenden.</rdfs:comment>
        <rdfs:comment xml:lang="en">The date the resource itself was put together. This is used to indicate a single date. For a date range use the property &apos;hasCreatedDate&apos;.</rdfs:comment>
        <rdfs:label xml:lang="en">has created date</rdfs:label>
        <skos:altLabel xml:lang="en">Date of creation</skos:altLabel>
        <skos:altLabel xml:lang="de">Erstellungsdatum</skos:altLabel>
    </owl:DatatypeProperty>
    


    <!-- &acdh;hasCreatedEndDate -->

    <owl:DatatypeProperty rdf:about="&acdh;hasCreatedEndDate">
        <rdfs:subPropertyOf rdf:resource="&acdh;hasDate"/>
        <rdfs:domain rdf:resource="&acdh;RepoObject"/>
        <rdfs:range rdf:resource="http://www.w3.org/2001/XMLSchema#date"/>
        <rdfs:comment xml:lang="de">Enddatum der Erstellung oder Zusammenstellung der Ressource oder Collection. Wird für die Angabe einer Zeitspanne verwendet. Ein einzelnes Datum wird mit der Eigenschaft &apos;hasCreatedDate&apos; angegeben.</rdfs:comment>
        <rdfs:comment xml:lang="en">The end date the resource itself was put together. This is used to indicate a date range. For a single date use the property &apos;hasCreatedDate&apos;.</rdfs:comment>
        <rdfs:label xml:lang="en">has created end date</rdfs:label>
        <skos:altLabel xml:lang="en">Date of creation (end)</skos:altLabel>
        <skos:altLabel xml:lang="de">Erstellungsdatum (Ende)</skos:altLabel>
    </owl:DatatypeProperty>
    


    <!-- &acdh;hasCreatedStartDate -->

    <owl:DatatypeProperty rdf:about="&acdh;hasCreatedStartDate">
        <rdfs:subPropertyOf rdf:resource="&acdh;hasDate"/>
        <rdfs:domain rdf:resource="&acdh;RepoObject"/>
        <rdfs:range rdf:resource="http://www.w3.org/2001/XMLSchema#date"/>
        <rdfs:comment xml:lang="de">Startdatum der Erstellung oder Zusammenstellung der Ressource oder Collection. Wird für die Angabe von Zeitspannen verwendet. Für ein einzelnes Datum die Eigenschaft &apos;hasCreatedDate&apos; verwenden.</rdfs:comment>
        <rdfs:comment xml:lang="en">The start date the resource itself was put together. This is used to indicate a date range. For a single date use the property &apos;hasCreatedDate&apos;.</rdfs:comment>
        <rdfs:label xml:lang="en">has created start date</rdfs:label>
        <skos:altLabel xml:lang="en">Date of creation (start)</skos:altLabel>
        <skos:altLabel xml:lang="de">Erstellungsdatum (Start)</skos:altLabel>
    </owl:DatatypeProperty>
    


    <!-- &acdh;hasDate -->

    <owl:DatatypeProperty rdf:about="&acdh;hasDate">
        <rdfs:subPropertyOf rdf:resource="http://www.w3.org/2002/07/owl#topDataProperty"/>
        <rdfs:range rdf:resource="http://www.w3.org/2001/XMLSchema#date"/>
        <rdfs:comment xml:lang="en">Date / point in time, either marking an event in the life cycle of an entity (Project, Collection or Resource) or used to describe temporal coverage of an entity (e.g. project dealing with historical texts from 17th century).</rdfs:comment>
        <rdfs:label xml:lang="en">has date</rdfs:label>
        <skos:altLabel xml:lang="en">Date</skos:altLabel>
        <skos:altLabel xml:lang="de">Datum</skos:altLabel>
    </owl:DatatypeProperty>
    


    <!-- &acdh;hasDescription -->

    <owl:DatatypeProperty rdf:about="&acdh;hasDescription">
        <rdfs:subPropertyOf rdf:resource="http://www.w3.org/2002/07/owl#topDataProperty"/>
        <rdfs:range rdf:resource="http://www.w3.org/2000/01/rdf-schema#Literal"/>
        <rdfs:comment xml:lang="en">A verbose description of certain aspects (content, coverage, completeness, extent, motivation, etc.) of an entity. This is the most generic property, use more specific sub-properties where applicable.</rdfs:comment>
        <rdfs:label xml:lang="en">has description</rdfs:label>
        <skos:altLabel xml:lang="de">Beschreibung</skos:altLabel>
        <skos:altLabel xml:lang="en">Description</skos:altLabel>
    </owl:DatatypeProperty>
    


    <!-- &acdh;hasEditorialPractice -->

    <owl:DatatypeProperty rdf:about="&acdh;hasEditorialPractice">
        <rdfs:subPropertyOf rdf:resource="&acdh;hasDescription"/>
        <rdfs:domain rdf:resource="&acdh;RepoObject"/>
        <rdfs:range rdf:resource="http://www.w3.org/2000/01/rdf-schema#Literal"/>
        <rdfs:comment xml:lang="en">Details of editorial principles and practices applied during the encoding of a text. Only relevant for digital editions.</rdfs:comment>
        <rdfs:label xml:lang="en">has editorial practice</rdfs:label>
        <skos:altLabel xml:lang="de">Angewendete editorische Praxis</skos:altLabel>
        <skos:altLabel xml:lang="en">Editorial practice used</skos:altLabel>
    </owl:DatatypeProperty>
    


    <!-- &acdh;hasEmail -->

    <owl:DatatypeProperty rdf:about="&acdh;hasEmail">
        <rdfs:subPropertyOf rdf:resource="&acdh;hasAddress"/>
        <rdfs:range rdf:resource="http://www.w3.org/2000/01/rdf-schema#Literal"/>
        <rdfs:comment xml:lang="en">E-mail associated with a Person or Organisation.</rdfs:comment>
        <rdfs:label xml:lang="en">has email</rdfs:label>
        <skos:altLabel xml:lang="de">E-Mail</skos:altLabel>
        <skos:altLabel xml:lang="en">E-mail</skos:altLabel>
    </owl:DatatypeProperty>
    


    <!-- &acdh;hasEndDate -->

    <owl:DatatypeProperty rdf:about="&acdh;hasEndDate">
        <rdfs:subPropertyOf rdf:resource="&acdh;hasDate"/>
        <rdfs:range rdf:resource="http://www.w3.org/2001/XMLSchema#date"/>
        <rdfs:comment xml:lang="en">Indicates the end date of a Project.</rdfs:comment>
        <rdfs:label xml:lang="en">has end date</rdfs:label>
        <skos:altLabel xml:lang="en">End date</skos:altLabel>
        <skos:altLabel xml:lang="de">Enddatum</skos:altLabel>
    </owl:DatatypeProperty>
    


    <!-- &acdh;hasEndpoint -->

    <owl:DatatypeProperty rdf:about="&acdh;hasEndpoint">
        <rdfs:subPropertyOf rdf:resource="http://www.w3.org/2002/07/owl#topDataProperty"/>
        <rdfs:domain rdf:resource="&acdh;RepoObject"/>
        <rdfs:range rdf:resource="http://www.w3.org/2001/XMLSchema#anyURI"/>
        <rdfs:comment xml:lang="en">URL of landing page. It should be created automatically by the system.</rdfs:comment>
        <rdfs:label xml:lang="en">has endpoint</rdfs:label>
        <skos:altLabel xml:lang="de">Endpoint</skos:altLabel>
        <skos:altLabel xml:lang="en">Endpoint</skos:altLabel>
    </owl:DatatypeProperty>
    


    <!-- &acdh;hasExtent -->

    <owl:DatatypeProperty rdf:about="&acdh;hasExtent">
        <rdfs:subPropertyOf rdf:resource="&acdh;hasDescription"/>
        <rdfs:domain rdf:resource="&acdh;RepoObject"/>
        <rdfs:range rdf:resource="http://www.w3.org/2000/01/rdf-schema#Literal"/>
        <rdfs:comment xml:lang="en">Indicates the extent (size or dimension) of a resource in any suitable measuring units.</rdfs:comment>
        <rdfs:label xml:lang="en">has extent</rdfs:label>
        <skos:altLabel xml:lang="de">Extent</skos:altLabel>
        <skos:altLabel xml:lang="en">Umfang</skos:altLabel>
    </owl:DatatypeProperty>
    


    <!-- &acdh;hasIdentifier -->

    <owl:DatatypeProperty rdf:about="&acdh;hasIdentifier">
        <rdfs:subPropertyOf rdf:resource="http://www.w3.org/2002/07/owl#topDataProperty"/>
        <rdfs:range rdf:resource="http://www.w3.org/2000/01/rdf-schema#Literal"/>
        <rdfs:comment xml:lang="en">Unique identifier given by ACDH and used in ACDH systems, as well as any other (internal) identifier assigned by other parties, e. g. a number assigned by the funder, an ID from another publication place or an inventory number.
Can be a literal in the form of prefix:identifier or can be an URI.
Handles belong into acdh:hasPID.</rdfs:comment>
        <rdfs:label xml:lang="en">has identifier</rdfs:label>
        <skos:altLabel xml:lang="en">Identifier</skos:altLabel>
        <skos:altLabel xml:lang="de">Identifikator</skos:altLabel>
    </owl:DatatypeProperty>
    


    <!-- &acdh;hasIssuedDate -->

    <owl:DatatypeProperty rdf:about="&acdh;hasIssuedDate">
        <rdfs:subPropertyOf rdf:resource="&acdh;hasDate"/>
        <rdfs:domain rdf:resource="&acdh;RepoObject"/>
        <rdfs:range rdf:resource="http://www.w3.org/2001/XMLSchema#date"/>
        <rdfs:comment xml:lang="de">Datum an dem die Ressource veröffentlicht oder verteilt wurde.</rdfs:comment>
        <rdfs:comment xml:lang="en">The date that the resource is published or distributed e.g. to a data centre.</rdfs:comment>
        <rdfs:label xml:lang="en">has issued date</rdfs:label>
        <skos:altLabel xml:lang="en">Date of Issue</skos:altLabel>
        <skos:altLabel xml:lang="de">Veröffentlichungsdatum</skos:altLabel>
    </owl:DatatypeProperty>
    


    <!-- &acdh;hasLatitude -->

    <owl:DatatypeProperty rdf:about="&acdh;hasLatitude">
        <rdfs:comment xml:lang="en">Geographic coordinate that specifies the north-south position of a point on the Earth&apos;s surface. Use signed degrees format (DD.dddd), e. g. -31.9600. Latitudes range from -90 to 90.</rdfs:comment>
        <rdfs:label xml:lang="en">has latitude</rdfs:label>
        <skos:altLabel xml:lang="de">Breitengrad</skos:altLabel>
        <skos:altLabel xml:lang="en">Latitude</skos:altLabel>
    </owl:DatatypeProperty>
    


    <!-- &acdh;hasLocationPath -->

    <owl:DatatypeProperty rdf:about="&acdh;hasLocationPath">
        <rdfs:subPropertyOf rdf:resource="http://www.w3.org/2002/07/owl#topDataProperty"/>
        <rdfs:domain rdf:resource="&acdh;RepoObject"/>
        <rdfs:range rdf:resource="http://www.w3.org/2000/01/rdf-schema#Literal"/>
        <rdfs:comment xml:lang="en">A filesystem path indicating the location from which a Collection or Resource was ingested. Used to match RepoObjects on re-ingest.</rdfs:comment>
        <rdfs:label xml:lang="en">has location path</rdfs:label>
        <skos:altLabel xml:lang="de">Dateipfad</skos:altLabel>
        <skos:altLabel xml:lang="en">File path</skos:altLabel>
    </owl:DatatypeProperty>
    


    <!-- &acdh;hasLongitude -->

    <owl:DatatypeProperty rdf:about="&acdh;hasLongitude">
        <rdfs:comment xml:lang="en">Geographic coordinate that specifies the east-west position of a point on the Earth&apos;s surface. Use signed degrees format (DDD.dddd), e. g. 115.8400. Longitudes range from -180 to 180.</rdfs:comment>
        <rdfs:label xml:lang="en">has longitude</rdfs:label>
        <skos:altLabel xml:lang="en">Longitude</skos:altLabel>
        <skos:altLabel xml:lang="de">Längengrad</skos:altLabel>
    </owl:DatatypeProperty>
    


    <!-- &acdh;hasNamingScheme -->

    <owl:DatatypeProperty rdf:about="&acdh;hasNamingScheme">
        <rdfs:subPropertyOf rdf:resource="&acdh;hasDescription"/>
        <rdfs:domain rdf:resource="&acdh;RepoObject"/>
        <rdfs:range rdf:resource="http://www.w3.org/2000/01/rdf-schema#Literal"/>
        <rdfs:comment xml:lang="en">Conventions used for naming and structuring of files and folders of the SIP.</rdfs:comment>
        <rdfs:label xml:lang="en">has naming scheme</rdfs:label>
        <skos:altLabel xml:lang="de">Beschreibung der verwendeten Namenskonventionen</skos:altLabel>
        <skos:altLabel xml:lang="en">Description of Naming Scheme used</skos:altLabel>
    </owl:DatatypeProperty>
    


    <!-- &acdh;hasNote -->

    <owl:DatatypeProperty rdf:about="&acdh;hasNote">
        <rdfs:subPropertyOf rdf:resource="&acdh;hasDescription"/>
        <rdfs:range rdf:resource="http://www.w3.org/2000/01/rdf-schema#Literal"/>
        <rdfs:comment xml:lang="en">Any other notes for the Project, Collection or Resource not fitting into an existing category. (DataCite: descriptionType Other)</rdfs:comment>
        <rdfs:label xml:lang="en">has note</rdfs:label>
        <skos:altLabel xml:lang="en">Note</skos:altLabel>
        <skos:altLabel xml:lang="de">Notiz</skos:altLabel>
    </owl:DatatypeProperty>
    


    <!-- &acdh;hasNumberOfItems -->

    <owl:DatatypeProperty rdf:about="&acdh;hasNumberOfItems">
        <rdfs:subPropertyOf rdf:resource="&acdh;hasDescription"/>
        <rdfs:domain rdf:resource="&acdh;RepoObject"/>
        <rdfs:range rdf:resource="http://www.w3.org/2001/XMLSchema#positiveInteger"/>
        <rdfs:comment xml:lang="en">Indicates the number of items (Resources) included in a Collection.</rdfs:comment>
        <rdfs:label xml:lang="en">has number of items</rdfs:label>
        <skos:altLabel xml:lang="en">Anzahl der Elemente</skos:altLabel>
        <skos:altLabel xml:lang="de">Number of items</skos:altLabel>
    </owl:DatatypeProperty>
    


    <!-- &acdh;hasPersonalTitle -->

    <owl:DatatypeProperty rdf:about="&acdh;hasPersonalTitle">
        <rdfs:domain rdf:resource="&acdh;Person"/>
        <rdfs:comment xml:lang="en">Professional or academic title of a Person.</rdfs:comment>
        <rdfs:label xml:lang="en">has personal title</rdfs:label>
        <skos:altLabel xml:lang="en">Titel</skos:altLabel>
        <skos:altLabel xml:lang="de">Title</skos:altLabel>
    </owl:DatatypeProperty>
    


    <!-- &acdh;hasPid -->

    <owl:DatatypeProperty rdf:about="&acdh;hasPid">
        <rdfs:subPropertyOf rdf:resource="http://www.w3.org/2002/07/owl#topDataProperty"/>
        <rdfs:comment xml:lang="en">Persistent identifier globally assigned to a Project, Collection or Resource. In ARCHE usually a Handle. A new Handle will be created if the identifier provided is non existent.
All other identifiers, like local assigned ones, project numbers or inventory numbers belong into acdh:hasIdentifier.</rdfs:comment>
        <rdfs:label xml:lang="en">has pid</rdfs:label>
        <skos:altLabel xml:lang="en">Persistent Identifier</skos:altLabel>
        <skos:altLabel xml:lang="de">Persistenter Identifikator</skos:altLabel>
    </owl:DatatypeProperty>
    


    <!-- &acdh;hasPostcode -->

    <owl:DatatypeProperty rdf:about="&acdh;hasPostcode">
        <rdfs:subPropertyOf rdf:resource="&acdh;hasAddress"/>
        <rdfs:range rdf:resource="http://www.w3.org/2000/01/rdf-schema#Literal"/>
        <rdfs:comment xml:lang="en">Postcode or zip code of adress associated with a Person or Organisation.</rdfs:comment>
        <rdfs:label xml:lang="en">has postcode</rdfs:label>
        <skos:altLabel xml:lang="en">Postcode/zip code</skos:altLabel>
        <skos:altLabel xml:lang="de">Postleitzahl</skos:altLabel>
    </owl:DatatypeProperty>
    


    <!-- &acdh;hasRegion -->

    <owl:DatatypeProperty rdf:about="&acdh;hasRegion">
        <rdfs:subPropertyOf rdf:resource="&acdh;hasAddress"/>
        <rdfs:range rdf:resource="http://www.w3.org/2000/01/rdf-schema#Literal"/>
        <rdfs:comment xml:lang="en">State, region or province of adress associated with a Person or Organisation.</rdfs:comment>
        <rdfs:label xml:lang="en">has region</rdfs:label>
        <skos:altLabel xml:lang="de">Staat/Region/Provinz</skos:altLabel>
        <skos:altLabel xml:lang="en">State/region/province</skos:altLabel>
    </owl:DatatypeProperty>
    


    <!-- &acdh;hasSeriesInformation -->

    <owl:DatatypeProperty rdf:about="&acdh;hasSeriesInformation">
        <rdfs:subPropertyOf rdf:resource="&acdh;hasDescription"/>
        <rdfs:domain rdf:resource="&acdh;RepoObject"/>
        <rdfs:range rdf:resource="http://www.w3.org/2000/01/rdf-schema#Literal"/>
        <rdfs:comment xml:lang="en">Information about a repeating series, such as volume, issue, number. For use with grey Literature. (DataCite descriptionType seriesInformation)</rdfs:comment>
        <rdfs:label xml:lang="en">has series information</rdfs:label>
        <skos:altLabel xml:lang="de">Informationen zur Reihe</skos:altLabel>
        <skos:altLabel xml:lang="en">Series information</skos:altLabel>
    </owl:DatatypeProperty>
    


    <!-- &acdh;hasStartDate -->

    <owl:DatatypeProperty rdf:about="&acdh;hasStartDate">
        <rdfs:subPropertyOf rdf:resource="&acdh;hasDate"/>
        <rdfs:range rdf:resource="http://www.w3.org/2001/XMLSchema#date"/>
        <rdfs:comment xml:lang="en">Indicates the start date of a Project.</rdfs:comment>
        <rdfs:label xml:lang="en">has start date</rdfs:label>
        <skos:altLabel xml:lang="de">Start date</skos:altLabel>
        <skos:altLabel xml:lang="de">Startdatum</skos:altLabel>
    </owl:DatatypeProperty>
    


    <!-- &acdh;hasSubmissionDate -->

    <owl:DatatypeProperty rdf:about="&acdh;hasSubmissionDate">
        <rdfs:subPropertyOf rdf:resource="&acdh;hasDate"/>
        <rdfs:range rdf:resource="http://www.w3.org/2001/XMLSchema#date"/>
        <rdfs:comment xml:lang="de">Datum an dem die Ressource vom Depositor übergeben wurde. Es kann sich von dem Annahmedatum unterscheiden, wenn ein Auswahlverfahren angewendet wird.</rdfs:comment>
        <rdfs:comment xml:lang="en">The date the depositor submits the resource to the repository. This could be different from acdh:hasAcceptedDate if the repository curator then applies a selection process.</rdfs:comment>
        <rdfs:label xml:lang="en">has submission date</rdfs:label>
        <skos:altLabel xml:lang="en">Date of submission</skos:altLabel>
        <skos:altLabel xml:lang="de">Einreichungsdatum</skos:altLabel>
    </owl:DatatypeProperty>
    


    <!-- &acdh;hasTableOfContents -->

    <owl:DatatypeProperty rdf:about="&acdh;hasTableOfContents">
        <rdfs:subPropertyOf rdf:resource="&acdh;hasDescription"/>
        <rdfs:domain rdf:resource="&acdh;RepoObject"/>
        <rdfs:range rdf:resource="http://www.w3.org/2000/01/rdf-schema#Literal"/>
        <rdfs:comment xml:lang="en">A listing of the Table of Contents. (DataCite: descriptionType tableOfContents)</rdfs:comment>
        <rdfs:label xml:lang="en">has table of contents</rdfs:label>
        <skos:altLabel xml:lang="de">Inhaltsverzeichnis</skos:altLabel>
        <skos:altLabel xml:lang="en">Table of contents</skos:altLabel>
    </owl:DatatypeProperty>
    


    <!-- &acdh;hasTechnicalInfo -->

    <owl:DatatypeProperty rdf:about="&acdh;hasTechnicalInfo">
        <rdfs:subPropertyOf rdf:resource="&acdh;hasDescription"/>
        <rdfs:domain rdf:resource="&acdh;RepoObject"/>
        <rdfs:range rdf:resource="http://www.w3.org/2000/01/rdf-schema#Literal"/>
        <rdfs:comment xml:lang="en">Detailed information that may be associated with design, implementation, operation, use, and/or maintenance of a process or system. (DataCite descriptionType technicalInfo)</rdfs:comment>
        <rdfs:label xml:lang="en">has technical info</rdfs:label>
        <skos:altLabel xml:lang="en">Technical information</skos:altLabel>
        <skos:altLabel xml:lang="de">Technische Informationen</skos:altLabel>
    </owl:DatatypeProperty>
    


    <!-- &acdh;hasTemporalCoverage -->

    <owl:DatatypeProperty rdf:about="&acdh;hasTemporalCoverage">
        <rdfs:comment xml:lang="en">Temporal coverage of content of Object, e.g. &apos;Roman&apos; for some archaeological data or &apos;1956-1965&apos; for a collection of digitised newspapers.</rdfs:comment>
        <rdfs:label xml:lang="en">has temporal coverage</rdfs:label>
        <skos:altLabel xml:lang="en">Has temporal coverage</skos:altLabel>
        <skos:altLabel xml:lang="de">Hat zeitliche Abdeckung</skos:altLabel>
    </owl:DatatypeProperty>
    


    <!-- &acdh;hasTitle -->

    <owl:DatatypeProperty rdf:about="&acdh;hasTitle">
        <rdfs:subPropertyOf rdf:resource="http://www.w3.org/2002/07/owl#topDataProperty"/>
        <rdfs:range rdf:resource="http://www.w3.org/2000/01/rdf-schema#Literal"/>
        <rdfs:comment xml:lang="en">Title or name of Project, Collection or Resource. Is also used as name for an organisation.</rdfs:comment>
        <rdfs:label xml:lang="en">has title</rdfs:label>
        <skos:altLabel xml:lang="de">Titel</skos:altLabel>
        <skos:altLabel xml:lang="en">Title</skos:altLabel>
    </owl:DatatypeProperty>
    


    <!-- &acdh;hasTransferDate -->

    <owl:DatatypeProperty rdf:about="&acdh;hasTransferDate">
        <rdfs:subPropertyOf rdf:resource="&acdh;hasDate"/>
        <rdfs:domain rdf:resource="&acdh;RepoObject"/>
        <rdfs:range rdf:resource="http://www.w3.org/2001/XMLSchema#date"/>
        <rdfs:comment xml:lang="en">Date of transfer of resources to the repository. Is asked for in the Deposition Agreement.</rdfs:comment>
        <rdfs:label xml:lang="en">has transfer date</rdfs:label>
        <skos:altLabel xml:lang="en">Date of transfer</skos:altLabel>
        <skos:altLabel xml:lang="de">Transferdatum</skos:altLabel>
    </owl:DatatypeProperty>
    


    <!-- &acdh;hasUpdatedDate -->

    <owl:DatatypeProperty rdf:about="&acdh;hasUpdatedDate">
        <rdfs:subPropertyOf rdf:resource="&acdh;hasDate"/>
        <rdfs:domain rdf:resource="&acdh;RepoObject"/>
        <rdfs:range rdf:resource="http://www.w3.org/2001/XMLSchema#date"/>
        <rdfs:comment xml:lang="de">Datum der letzten Aktualisierung.</rdfs:comment>
        <rdfs:comment xml:lang="en">The date of the last update/change to the resource.</rdfs:comment>
        <rdfs:label xml:lang="en">has updated date</rdfs:label>
        <skos:altLabel xml:lang="en">Date of last update</skos:altLabel>
        <skos:altLabel xml:lang="de">Datum der letzten Aktualisierung</skos:altLabel>
    </owl:DatatypeProperty>
    


    <!-- &acdh;hasUrl -->

    <owl:DatatypeProperty rdf:about="&acdh;hasUrl">
        <rdfs:subPropertyOf rdf:resource="http://www.w3.org/2002/07/owl#topDataProperty"/>
        <rdfs:domain rdf:resource="&acdh;RepoObject"/>
        <rdfs:range rdf:resource="http://www.w3.org/2001/XMLSchema#anyURI"/>
        <rdfs:comment xml:lang="en">Used to add URLs to for organisations, agents, projects etc.</rdfs:comment>
        <rdfs:label xml:lang="en">has url</rdfs:label>
        <skos:altLabel xml:lang="de">URL</skos:altLabel>
        <skos:altLabel xml:lang="en">URL</skos:altLabel>
    </owl:DatatypeProperty>
    


    <!-- &acdh;hasUsedHardware -->

    <owl:DatatypeProperty rdf:about="&acdh;hasUsedHardware">
        <rdfs:comment xml:lang="en">Hardware used for creating or processing the Resource. Provide name including model numbers, versions etc.</rdfs:comment>
        <rdfs:label xml:lang="en">has used hardware</rdfs:label>
        <skos:altLabel xml:lang="de">Hardware</skos:altLabel>
        <skos:altLabel xml:lang="en">Hardware</skos:altLabel>
    </owl:DatatypeProperty>
    


    <!-- &acdh;hasUsedSoftware -->

    <owl:DatatypeProperty rdf:about="&acdh;hasUsedSoftware">
        <rdfs:comment xml:lang="en">Software used for creating or processing of the Resource. Provide name of software and version used.</rdfs:comment>
        <rdfs:label xml:lang="en">has used software</rdfs:label>
        <skos:altLabel xml:lang="de">Software</skos:altLabel>
        <skos:altLabel xml:lang="en">Software</skos:altLabel>
    </owl:DatatypeProperty>
    


    <!-- &acdh;hasValidEndDate -->

    <owl:DatatypeProperty rdf:about="&acdh;hasValidEndDate">
        <rdfs:subPropertyOf rdf:resource="&acdh;hasDate"/>
        <rdfs:domain rdf:resource="&acdh;RepoObject"/>
        <rdfs:range rdf:resource="http://www.w3.org/2001/XMLSchema#date"/>
        <rdfs:comment xml:lang="de">Datum oder Zeitraum in dem der Inhalt der Ressource gültig ist. Enddatum.</rdfs:comment>
        <rdfs:comment xml:lang="en">The date or date range during which the dataset or resource is accurate. End date.</rdfs:comment>
        <rdfs:label xml:lang="en">has valid end date</rdfs:label>
        <skos:altLabel xml:lang="en">Date of validity (end)</skos:altLabel>
        <skos:altLabel xml:lang="de">Gültigkeitsdatum (Ende)</skos:altLabel>
    </owl:DatatypeProperty>
    


    <!-- &acdh;hasValidStartDate -->

    <owl:DatatypeProperty rdf:about="&acdh;hasValidStartDate">
        <rdfs:subPropertyOf rdf:resource="&acdh;hasDate"/>
        <rdfs:domain rdf:resource="&acdh;RepoObject"/>
        <rdfs:range rdf:resource="http://www.w3.org/2001/XMLSchema#date"/>
        <rdfs:comment xml:lang="de">Datum oder Zeitraum in dem der Inhalt der Ressource gültig ist. Startdatum.</rdfs:comment>
        <rdfs:comment xml:lang="en">The date or date range during which the dataset or resource is accurate. Start date.</rdfs:comment>
        <rdfs:label xml:lang="en">has valid start date</rdfs:label>
        <skos:altLabel xml:lang="en">Date of validity (start)</skos:altLabel>
        <skos:altLabel xml:lang="de">Gültigkeitsdatum (Start)</skos:altLabel>
    </owl:DatatypeProperty>
    


    <!-- &acdh;hasVersion -->

    <owl:DatatypeProperty rdf:about="&acdh;hasVersion">
        <rdfs:subPropertyOf rdf:resource="http://www.w3.org/2002/07/owl#topDataProperty"/>
        <rdfs:comment xml:lang="en">Number of name of the version of Collection or Resource.</rdfs:comment>
        <rdfs:label xml:lang="en">has version</rdfs:label>
        <skos:altLabel xml:lang="de">Version</skos:altLabel>
        <skos:altLabel xml:lang="en">Version</skos:altLabel>
    </owl:DatatypeProperty>
    


    <!-- &acdh;hasWKT -->

    <owl:DatatypeProperty rdf:about="&acdh;hasWKT">
        <rdfs:comment xml:lang="en">Well-known text (WKT) of a Place for representation on a map. WKT is defined by ISO 19162. Wicket might be used to create valid WKT: http://arthur-e.github.io/Wicket/sandbox-gmaps3.html</rdfs:comment>
        <rdfs:label xml:lang="en">has wkt</rdfs:label>
        <skos:altLabel xml:lang="de">WKT</skos:altLabel>
        <skos:altLabel xml:lang="en">WKT</skos:altLabel>
    </owl:DatatypeProperty>
    


    <!-- &acdh;language -->

    <owl:DatatypeProperty rdf:about="&acdh;language">
        <rdfs:domain rdf:resource="&acdh;RepoObject"/>
        <rdfs:range rdf:resource="http://www.w3.org/2001/XMLSchema#language"/>
        <rdfs:comment xml:lang="en">Language of Collection or Resource. Ideally encoded with 3-letter code according to ISO-639-3 (e.g. deu, eng, arz)</rdfs:comment>
        <rdfs:label xml:lang="en">has language</rdfs:label>
        <skos:altLabel xml:lang="de">Language</skos:altLabel>
        <skos:altLabel xml:lang="en">Sprache</skos:altLabel>
    </owl:DatatypeProperty>
    


    <!-- 
    ///////////////////////////////////////////////////////////////////////////////////////
    //
    // Classes
    //
    ///////////////////////////////////////////////////////////////////////////////////////
     -->

    


    <!-- http://www.w3.org/2004/02/skos/core#Concept -->

    <owl:Class rdf:about="http://www.w3.org/2004/02/skos/core#Concept">
        <owl:equivalentClass rdf:resource="&acdh;Concept"/>
    </owl:Class>
    


    <!-- http://xmlns.com/foaf/0.1/Agent -->

    <owl:Class rdf:about="http://xmlns.com/foaf/0.1/Agent"/>
    


    <!-- http://xmlns.com/foaf/0.1/Organization -->

    <owl:Class rdf:about="http://xmlns.com/foaf/0.1/Organization">
        <owl:equivalentClass rdf:resource="&acdh;Organisation"/>
        <rdfs:subClassOf rdf:resource="http://xmlns.com/foaf/0.1/Agent"/>
    </owl:Class>
    


    <!-- http://xmlns.com/foaf/0.1/Person -->

    <owl:Class rdf:about="http://xmlns.com/foaf/0.1/Person">
        <owl:equivalentClass rdf:resource="&acdh;Person"/>
        <rdfs:subClassOf rdf:resource="http://xmlns.com/foaf/0.1/Agent"/>
    </owl:Class>
    


    <!-- http://xmlns.com/foaf/0.1/Project -->

    <owl:Class rdf:about="http://xmlns.com/foaf/0.1/Project">
        <owl:equivalentClass rdf:resource="&acdh;Project"/>
    </owl:Class>
    


    <!-- &acdh;Agent -->

    <owl:Class rdf:about="&acdh;Agent">
        <rdfs:subClassOf rdf:resource="http://www.w3.org/2002/07/owl#Thing"/>
        <rdfs:subClassOf>
            <owl:Restriction>
                <owl:onProperty rdf:resource="&acdh;hasAddressLine1"/>
                <owl:minCardinality rdf:datatype="http://www.w3.org/2001/XMLSchema#nonNegativeInteger">0</owl:minCardinality>
            </owl:Restriction>
        </rdfs:subClassOf>
        <rdfs:subClassOf>
            <owl:Restriction>
                <owl:onProperty rdf:resource="&acdh;hasAddressLine2"/>
                <owl:minCardinality rdf:datatype="http://www.w3.org/2001/XMLSchema#nonNegativeInteger">0</owl:minCardinality>
            </owl:Restriction>
        </rdfs:subClassOf>
        <rdfs:subClassOf>
            <owl:Restriction>
                <owl:onProperty rdf:resource="&acdh;hasCity"/>
                <owl:minCardinality rdf:datatype="http://www.w3.org/2001/XMLSchema#nonNegativeInteger">0</owl:minCardinality>
            </owl:Restriction>
        </rdfs:subClassOf>
        <rdfs:subClassOf>
            <owl:Restriction>
                <owl:onProperty rdf:resource="&acdh;hasCountry"/>
                <owl:minCardinality rdf:datatype="http://www.w3.org/2001/XMLSchema#nonNegativeInteger">0</owl:minCardinality>
            </owl:Restriction>
        </rdfs:subClassOf>
        <rdfs:subClassOf>
            <owl:Restriction>
                <owl:onProperty rdf:resource="&acdh;hasEmail"/>
                <owl:minCardinality rdf:datatype="http://www.w3.org/2001/XMLSchema#nonNegativeInteger">0</owl:minCardinality>
            </owl:Restriction>
        </rdfs:subClassOf>
        <rdfs:subClassOf>
            <owl:Restriction>
                <owl:onProperty rdf:resource="&acdh;hasPostcode"/>
                <owl:minCardinality rdf:datatype="http://www.w3.org/2001/XMLSchema#nonNegativeInteger">0</owl:minCardinality>
            </owl:Restriction>
        </rdfs:subClassOf>
        <rdfs:subClassOf>
            <owl:Restriction>
                <owl:onProperty rdf:resource="&acdh;hasRegion"/>
                <owl:minCardinality rdf:datatype="http://www.w3.org/2001/XMLSchema#nonNegativeInteger">0</owl:minCardinality>
            </owl:Restriction>
        </rdfs:subClassOf>
        <rdfs:subClassOf>
            <owl:Restriction>
                <owl:onProperty rdf:resource="&acdh;hasUrl"/>
                <owl:minQualifiedCardinality rdf:datatype="http://www.w3.org/2001/XMLSchema#nonNegativeInteger">0</owl:minQualifiedCardinality>
                <owl:onDataRange rdf:resource="http://www.w3.org/2001/XMLSchema#anyURI"/>
            </owl:Restriction>
        </rdfs:subClassOf>
        <rdfs:comment xml:lang="en">Entity able to act, in the context of this schema especially be involved in the making, processing, distributing, publishing etc. of a Resource, Collection, Concept or Project.
Note that in contrast to foaf:Agent acdh:Agent can only be a Person or an Organisation (not a software or physical artifact).
The different roles an Agent can assume with respect to a Project, Collection, Resource or Concept are modeled as separate object properties (sub-properties of acdh:contributedTo).</rdfs:comment>
        <rdfs:label xml:lang="en">Agent</rdfs:label>
        <skos:altLabel xml:lang="en">Agent</skos:altLabel>
        <skos:altLabel xml:lang="de">Akteur</skos:altLabel>
    </owl:Class>
    


    <!-- &acdh;Collection -->

    <owl:Class rdf:about="&acdh;Collection">
        <rdfs:subClassOf rdf:resource="&acdh;RepoObject"/>
        <rdfs:subClassOf>
            <owl:Restriction>
                <owl:onProperty rdf:resource="&acdh;hasContributor"/>
                <owl:minQualifiedCardinality rdf:datatype="http://www.w3.org/2001/XMLSchema#nonNegativeInteger">1</owl:minQualifiedCardinality>
                <owl:onClass rdf:resource="&acdh;Agent"/>
            </owl:Restriction>
        </rdfs:subClassOf>
        <rdfs:subClassOf>
            <owl:Restriction>
                <owl:onProperty rdf:resource="&acdh;hasSubject"/>
                <owl:minCardinality rdf:datatype="http://www.w3.org/2001/XMLSchema#nonNegativeInteger">1</owl:minCardinality>
            </owl:Restriction>
        </rdfs:subClassOf>
        <rdfs:comment xml:lang="en">Set of Repo Objects (Collections or Resources), much like folders in a file system. A Collection can be optionally related to a Project (acdh:hasRelatedProject), in which it was created or curated.</rdfs:comment>
        <rdfs:label xml:lang="en">Collection</rdfs:label>
        <skos:altLabel xml:lang="en">Collection</skos:altLabel>
        <skos:altLabel xml:lang="de">Sammlung</skos:altLabel>
    </owl:Class>
    


    <!-- &acdh;Concept -->

    <owl:Class rdf:about="&acdh;Concept">
        <rdfs:subClassOf rdf:resource="http://www.w3.org/2002/07/owl#Thing"/>
        <rdfs:comment xml:lang="en">This class is equivalent to skos:Concept: A SKOS concept can be viewed as an idea or notion; a unit of thought. The notion of a SKOS concept is useful when describing the conceptual or intellectual structure of a knowledge organization system, and when referring to specific ideas or meanings established within a KOS. (source: https://www.w3.org/TR/skos-reference/#concepts)
This class is used to link controlled lists stored in SKOS format to object or data properties. E. g. a list of possible resource types for acdh:hasCategory.</rdfs:comment>
        <rdfs:label xml:lang="en">Concept</rdfs:label>
        <skos:altLabel xml:lang="en">Concept</skos:altLabel>
        <skos:altLabel xml:lang="de">Konzept</skos:altLabel>
    </owl:Class>
    


    <!-- &acdh;Image -->

    <owl:Class rdf:about="&acdh;Image">
        <rdfs:subClassOf rdf:resource="&acdh;RepoObject"/>
        <rdfs:comment xml:lang="en">An image used for presentation of a related Repo Object. It should only be used for logos and title images. Images in data sets are use the class Resource.</rdfs:comment>
        <rdfs:label xml:lang="en">Image</rdfs:label>
        <skos:altLabel xml:lang="de">Bild</skos:altLabel>
        <skos:altLabel xml:lang="en">Image</skos:altLabel>
    </owl:Class>
    


    <!-- &acdh;Metadata -->

    <owl:Class rdf:about="&acdh;Metadata">
        <rdfs:subClassOf rdf:resource="&acdh;RepoObject"/>
        <rdfs:comment xml:lang="en">Structured information in form of a separate binary file ABOUT another Repo Object. 
The Metadata object is linked to the RepoObject it describes with the relation acdh:hasMetadata.
The default example is a CMDI file that describes other resources.</rdfs:comment>
        <rdfs:label xml:lang="en">Metadata</rdfs:label>
        <skos:altLabel xml:lang="en">Metadata</skos:altLabel>
        <skos:altLabel xml:lang="de">Metadaten</skos:altLabel>
    </owl:Class>
    


    <!-- &acdh;Organisation -->

    <owl:Class rdf:about="&acdh;Organisation">
        <rdfs:subClassOf rdf:resource="&acdh;Agent"/>
        <rdfs:subClassOf>
            <owl:Restriction>
                <owl:onProperty rdf:resource="&acdh;hasAlternativeTitle"/>
                <owl:minCardinality rdf:datatype="http://www.w3.org/2001/XMLSchema#nonNegativeInteger">0</owl:minCardinality>
            </owl:Restriction>
        </rdfs:subClassOf>
        <rdfs:subClassOf>
            <owl:Restriction>
                <owl:onProperty rdf:resource="&acdh;hasIdentifier"/>
                <owl:minCardinality rdf:datatype="http://www.w3.org/2001/XMLSchema#nonNegativeInteger">1</owl:minCardinality>
            </owl:Restriction>
        </rdfs:subClassOf>
        <rdfs:subClassOf>
            <owl:Restriction>
                <owl:onProperty rdf:resource="&acdh;hasTitle"/>
                <owl:cardinality rdf:datatype="http://www.w3.org/2001/XMLSchema#nonNegativeInteger">1</owl:cardinality>
            </owl:Restriction>
        </rdfs:subClassOf>
        <rdfs:comment xml:lang="en">A legal entity (university, company) or its organisational substructure (department, institute), related in some way to a Project, Collection or Resource. The nature of the relation is specified by designated object properties, as described in the super-class acdh:Agent.</rdfs:comment>
        <rdfs:comment>[Martina: will need a name (hasTitle?), a place (property? spatialCoverage does not fit; maybe hasAddress?), a URL, a Phone, identifiers, a logo]</rdfs:comment>
        <rdfs:label xml:lang="en">Organisation</rdfs:label>
        <skos:altLabel xml:lang="de">Organisation oder Institution</skos:altLabel>
        <skos:altLabel xml:lang="en">Organisation or Institution</skos:altLabel>
    </owl:Class>
    


    <!-- &acdh;Person -->

    <owl:Class rdf:about="&acdh;Person">
        <rdfs:subClassOf rdf:resource="&acdh;Agent"/>
        <rdfs:subClassOf>
            <owl:Restriction>
                <owl:onProperty rdf:resource="&acdh;isMember"/>
                <owl:someValuesFrom rdf:resource="&acdh;Organisation"/>
            </owl:Restriction>
        </rdfs:subClassOf>
        <rdfs:subClassOf>
            <owl:Restriction>
                <owl:onProperty rdf:resource="http://vocabs.acdh.oeaw.ac.at#hasFirstName"/>
                <owl:minCardinality rdf:datatype="http://www.w3.org/2001/XMLSchema#nonNegativeInteger">0</owl:minCardinality>
            </owl:Restriction>
        </rdfs:subClassOf>
        <rdfs:subClassOf>
            <owl:Restriction>
                <owl:onProperty rdf:resource="http://vocabs.acdh.oeaw.ac.at#hasLastName"/>
                <owl:minCardinality rdf:datatype="http://www.w3.org/2001/XMLSchema#nonNegativeInteger">1</owl:minCardinality>
            </owl:Restriction>
        </rdfs:subClassOf>
        <rdfs:subClassOf>
            <owl:Restriction>
                <owl:onProperty rdf:resource="&acdh;hasIdentifier"/>
                <owl:minCardinality rdf:datatype="http://www.w3.org/2001/XMLSchema#nonNegativeInteger">0</owl:minCardinality>
            </owl:Restriction>
        </rdfs:subClassOf>
        <rdfs:subClassOf>
            <owl:Restriction>
                <owl:onProperty rdf:resource="&acdh;hasPersonalTitle"/>
                <owl:minCardinality rdf:datatype="http://www.w3.org/2001/XMLSchema#nonNegativeInteger">0</owl:minCardinality>
            </owl:Restriction>
        </rdfs:subClassOf>
        <rdfs:comment xml:lang="en">An individual related in some way to a Project, Collection or Resource. 
The nature of the relation is specified by designated object properties as described in the super-class acdh:Agent.
A Person can be linked to an Organisation by using isMember.</rdfs:comment>
        <rdfs:comment>[Martina: will also need title (e.g. dr. prof.), e-mail, phone, address, identifier (0-*), relation to organisation (1-*)]</rdfs:comment>
        <rdfs:label xml:lang="en">Person</rdfs:label>
        <skos:altLabel xml:lang="de">Person</skos:altLabel>
        <skos:altLabel xml:lang="en">Person</skos:altLabel>
    </owl:Class>
    


    <!-- &acdh;Place -->

    <owl:Class rdf:about="&acdh;Place">
        <rdfs:subClassOf rdf:resource="http://www.w3.org/2002/07/owl#Thing"/>
        <rdfs:subClassOf>
            <owl:Restriction>
                <owl:onProperty rdf:resource="&acdh;hasAlternativeTitle"/>
                <owl:minCardinality rdf:datatype="http://www.w3.org/2001/XMLSchema#nonNegativeInteger">0</owl:minCardinality>
            </owl:Restriction>
        </rdfs:subClassOf>
        <rdfs:subClassOf>
            <owl:Restriction>
                <owl:onProperty rdf:resource="&acdh;hasIdentifier"/>
                <owl:minCardinality rdf:datatype="http://www.w3.org/2001/XMLSchema#nonNegativeInteger">0</owl:minCardinality>
            </owl:Restriction>
        </rdfs:subClassOf>
        <rdfs:subClassOf>
            <owl:Restriction>
                <owl:onProperty rdf:resource="&acdh;hasTitle"/>
                <owl:cardinality rdf:datatype="http://www.w3.org/2001/XMLSchema#nonNegativeInteger">1</owl:cardinality>
            </owl:Restriction>
        </rdfs:subClassOf>
        <rdfs:subClassOf>
            <owl:Restriction>
                <owl:onProperty rdf:resource="&acdh;hasLatitude"/>
                <owl:maxQualifiedCardinality rdf:datatype="http://www.w3.org/2001/XMLSchema#nonNegativeInteger">1</owl:maxQualifiedCardinality>
                <owl:onDataRange rdf:resource="http://www.w3.org/2001/XMLSchema#float"/>
            </owl:Restriction>
        </rdfs:subClassOf>
        <rdfs:subClassOf>
            <owl:Restriction>
                <owl:onProperty rdf:resource="&acdh;hasLongitude"/>
                <owl:maxQualifiedCardinality rdf:datatype="http://www.w3.org/2001/XMLSchema#nonNegativeInteger">1</owl:maxQualifiedCardinality>
                <owl:onDataRange rdf:resource="http://www.w3.org/2001/XMLSchema#float"/>
            </owl:Restriction>
        </rdfs:subClassOf>
        <rdfs:subClassOf>
            <owl:Restriction>
                <owl:onProperty rdf:resource="&acdh;hasWKT"/>
                <owl:maxCardinality rdf:datatype="http://www.w3.org/2001/XMLSchema#nonNegativeInteger">1</owl:maxCardinality>
            </owl:Restriction>
        </rdfs:subClassOf>
        <rdfs:comment xml:lang="en">A Place represents a geographical location. It can be used to indicate the spatial coverage of a Project, Collection or Resource, as well as to describe the publishing place of a work. It should contain information about the name, geocoordinates and identifiers to refer to existing gazetteers.</rdfs:comment>
        <rdfs:comment>[Martina: needs name; alternativeName(s); country code; long and lat or wkt; identifier(s)
what to do if continents should be used as place?
relations (properties): more than only spatialCoverage
]</rdfs:comment>
        <rdfs:label xml:lang="en">Place</rdfs:label>
        <skos:altLabel xml:lang="de">Ort</skos:altLabel>
        <skos:altLabel xml:lang="en">Place</skos:altLabel>
    </owl:Class>
    


    <!-- &acdh;Project -->

    <owl:Class rdf:about="&acdh;Project">
        <rdfs:subClassOf rdf:resource="http://www.w3.org/2002/07/owl#Thing"/>
        <rdfs:subClassOf>
            <owl:Restriction>
                <owl:onProperty rdf:resource="&acdh;hasPrincipalInvestigator"/>
                <owl:minQualifiedCardinality rdf:datatype="http://www.w3.org/2001/XMLSchema#nonNegativeInteger">0</owl:minQualifiedCardinality>
                <owl:onClass rdf:resource="&acdh;Agent"/>
            </owl:Restriction>
        </rdfs:subClassOf>
        <rdfs:subClassOf>
            <owl:Restriction>
                <owl:onProperty rdf:resource="&acdh;hasSubject"/>
                <owl:minQualifiedCardinality rdf:datatype="http://www.w3.org/2001/XMLSchema#nonNegativeInteger">1</owl:minQualifiedCardinality>
                <owl:onClass rdf:resource="&acdh;Concept"/>
            </owl:Restriction>
        </rdfs:subClassOf>
        <rdfs:subClassOf>
            <owl:Restriction>
                <owl:onProperty rdf:resource="&acdh;hasAlternativeTitle"/>
                <owl:minCardinality rdf:datatype="http://www.w3.org/2001/XMLSchema#nonNegativeInteger">0</owl:minCardinality>
            </owl:Restriction>
        </rdfs:subClassOf>
        <rdfs:subClassOf>
            <owl:Restriction>
                <owl:onProperty rdf:resource="&acdh;hasDescription"/>
                <owl:minCardinality rdf:datatype="http://www.w3.org/2001/XMLSchema#nonNegativeInteger">1</owl:minCardinality>
            </owl:Restriction>
        </rdfs:subClassOf>
        <rdfs:subClassOf>
            <owl:Restriction>
                <owl:onProperty rdf:resource="&acdh;hasIdentifier"/>
                <owl:minCardinality rdf:datatype="http://www.w3.org/2001/XMLSchema#nonNegativeInteger">0</owl:minCardinality>
            </owl:Restriction>
        </rdfs:subClassOf>
        <rdfs:subClassOf>
            <owl:Restriction>
                <owl:onProperty rdf:resource="&acdh;language"/>
                <owl:minQualifiedCardinality rdf:datatype="http://www.w3.org/2001/XMLSchema#nonNegativeInteger">1</owl:minQualifiedCardinality>
                <owl:onDataRange rdf:resource="http://www.w3.org/2001/XMLSchema#language"/>
            </owl:Restriction>
        </rdfs:subClassOf>
        <rdfs:subClassOf>
            <owl:Restriction>
                <owl:onProperty rdf:resource="&acdh;hasTitle"/>
                <owl:cardinality rdf:datatype="http://www.w3.org/2001/XMLSchema#nonNegativeInteger">1</owl:cardinality>
            </owl:Restriction>
        </rdfs:subClassOf>
        <rdfs:comment xml:lang="en">Effort or activity with defined goals and (normally) limited time scope, usually in collaborative setup with dedicated funding.</rdfs:comment>
        <rdfs:comment xml:lang="en">Note that though a Project might (and usually will) use or produce data, it is NOT modelled as a Collection (of data). Thus the relation between the data and the Project is acdh:hasRelatedProject NOT acdh:partOf.</rdfs:comment>
        <rdfs:comment>[Martina: needs a property for start and end date]</rdfs:comment>
        <rdfs:label xml:lang="en">Project</rdfs:label>
        <skos:altLabel xml:lang="en">Project</skos:altLabel>
        <skos:altLabel xml:lang="de">Projekt</skos:altLabel>
    </owl:Class>
    


    <!-- &acdh;Publication -->

    <owl:Class rdf:about="&acdh;Publication">
        <rdfs:subClassOf rdf:resource="&acdh;Resource"/>
        <rdfs:comment xml:lang="en">Verbose research output like a journal article, paper submitted to a conference, a book  etc. In this schema primarily intended to allow capturing publications related to certain Projects, Collections or Resources.</rdfs:comment>
        <rdfs:label xml:lang="en">Publication</rdfs:label>
        <skos:altLabel xml:lang="en">Publication</skos:altLabel>
        <skos:altLabel xml:lang="de">Publikation</skos:altLabel>
    </owl:Class>
    


    <!-- &acdh;RepoObject -->

    <owl:Class rdf:about="&acdh;RepoObject">
        <rdfs:subClassOf rdf:resource="http://www.w3.org/2002/07/owl#Thing"/>
        <rdfs:subClassOf>
            <owl:Restriction>
                <owl:onProperty rdf:resource="&acdh;hasCategory"/>
                <owl:minCardinality rdf:datatype="http://www.w3.org/2001/XMLSchema#nonNegativeInteger">1</owl:minCardinality>
            </owl:Restriction>
        </rdfs:subClassOf>
        <rdfs:subClassOf>
            <owl:Restriction>
                <owl:onProperty rdf:resource="&acdh;hasHosting"/>
                <owl:minQualifiedCardinality rdf:datatype="http://www.w3.org/2001/XMLSchema#nonNegativeInteger">1</owl:minQualifiedCardinality>
                <owl:onClass rdf:resource="&acdh;Organisation"/>
            </owl:Restriction>
        </rdfs:subClassOf>
        <rdfs:subClassOf>
            <owl:Restriction>
                <owl:onProperty rdf:resource="&acdh;hasLicense"/>
                <owl:cardinality rdf:datatype="http://www.w3.org/2001/XMLSchema#nonNegativeInteger">1</owl:cardinality>
            </owl:Restriction>
        </rdfs:subClassOf>
        <rdfs:subClassOf>
            <owl:Restriction>
                <owl:onProperty rdf:resource="&acdh;hasRightsHolder"/>
                <owl:qualifiedCardinality rdf:datatype="http://www.w3.org/2001/XMLSchema#nonNegativeInteger">1</owl:qualifiedCardinality>
                <owl:onClass rdf:resource="&acdh;Agent"/>
            </owl:Restriction>
        </rdfs:subClassOf>
        <rdfs:subClassOf>
            <owl:Restriction>
                <owl:onProperty rdf:resource="&acdh;hasTitle"/>
                <owl:minCardinality rdf:datatype="http://www.w3.org/2001/XMLSchema#nonNegativeInteger">1</owl:minCardinality>
            </owl:Restriction>
        </rdfs:subClassOf>
        <rdfs:subClassOf>
            <owl:Restriction>
                <owl:onProperty rdf:resource="&acdh;language"/>
                <owl:minQualifiedCardinality rdf:datatype="http://www.w3.org/2001/XMLSchema#nonNegativeInteger">1</owl:minQualifiedCardinality>
                <owl:onDataRange rdf:resource="http://www.w3.org/2001/XMLSchema#language"/>
            </owl:Restriction>
        </rdfs:subClassOf>
        <rdfs:subClassOf>
            <owl:Restriction>
                <owl:onProperty rdf:resource="&acdh;hasIdentifier"/>
                <owl:cardinality rdf:datatype="http://www.w3.org/2001/XMLSchema#nonNegativeInteger">1</owl:cardinality>
            </owl:Restriction>
        </rdfs:subClassOf>
        <rdfs:subClassOf>
            <owl:Restriction>
                <owl:onProperty rdf:resource="&acdh;hasAvailableDate"/>
                <owl:maxQualifiedCardinality rdf:datatype="http://www.w3.org/2001/XMLSchema#nonNegativeInteger">1</owl:maxQualifiedCardinality>
                <owl:onDataRange rdf:resource="http://www.w3.org/2001/XMLSchema#date"/>
            </owl:Restriction>
        </rdfs:subClassOf>
        <rdfs:subClassOf>
            <owl:Restriction>
                <owl:onProperty rdf:resource="&acdh;hasVersion"/>
                <owl:maxCardinality rdf:datatype="http://www.w3.org/2001/XMLSchema#nonNegativeInteger">1</owl:maxCardinality>
            </owl:Restriction>
        </rdfs:subClassOf>
        <rdfs:comment xml:lang="en">Generic entity representing the items in the repository - Collections and Resources, which are modelled as subclasses of Repo Object.</rdfs:comment>
        <rdfs:comment xml:lang="en">Note that other classes, especially Project, are not considered subclasses of Repo Object.</rdfs:comment>
        <rdfs:label>Repo Object</rdfs:label>
    </owl:Class>
    


    <!-- &acdh;Resource -->

    <owl:Class rdf:about="&acdh;Resource">
        <rdfs:subClassOf rdf:resource="&acdh;RepoObject"/>
        <rdfs:comment xml:lang="en">Basic entity in the schema containing actual data / content payload; comparable (and mostly equivalent) to files in a file system.</rdfs:comment>
        <rdfs:label xml:lang="en">Resource</rdfs:label>
        <skos:altLabel xml:lang="en">Resource</skos:altLabel>
        <skos:altLabel xml:lang="de">Ressource</skos:altLabel>
    </owl:Class>
</rdf:RDF>



<!-- Generated by the OWL API (version 4.2.8.20170104-2310) https://github.com/owlcs/owlapi -->

